Remove [Membership]

theories/Alpha.v
@@ -3,7 +3,6 @@
 
    ===== TODOs =====
    These will probably be rendered moot by [compute-sets] (assuming it is a success):
-     - Remove [bool]/[Prop] output distinctions (e.g. [\in] vs [∈])?
      - Remove unnecessary casts.
      - Standardize naming for [domm], [codomm], [co_domm], [co_domain], etc.
      - Create specialized versions of lemmas that use e.g. [domm f] instead of [X] and [codomm_Tm_set f] instead of [Y].
@@ -20,8 +19,7 @@
    These are specific to [compute-sets]:
      - Change all the [*_type] proofs to talk about [domm] and [codomm], and re-add any that were removed from this branch despite being referenced in the paper.
      - Use boolean implication instead of [->] where possible?
-     - Remove [Membership]?
-     - Use [t ∈ Tm X] instead of [FV t ⊆ Tm X]. *)
+     - Set [getmP], [imfsetP], etc. to have implicit arguments (for consistency)? *)
 
 From Coq Require Import Classes.RelationClasses Lists.List Program.Equality Setoid ssreflect.
 From mathcomp Require Import bigop choice eqtype seq ssrbool ssrfun ssrnat.
@@ -81,7 +79,7 @@ Module AlphaFacts (Import M : Alpha).
 
     Inductive in_Tm : {fset 𝒱} -> term -> Prop :=
     | Tm_variable : forall X x,
-        x ∈ X : Prop ->
+        x ∈ X ->
         variable x ∈ Tm X
     | Tm_application : forall X t u,
         t ∈ Tm X -> u ∈ Tm X ->
@@ -97,27 +95,19 @@ Module AlphaFacts (Import M : Alpha).
 
   Lemma TmP : forall X t, reflect (in_Tm X t) (t ∈ Tm X).
   Proof.
-    rewrite /Tm /=.
+    rewrite /Tm /in_mem /=.
     intros.
-    gen X. induction t; intros;
-    rewrite /in_mem /=;
+    gen X. induction t; intros; simpl;
     ((rewrite fsubD1set fsetUC; destruct (IHt (X ∪ {s}))) ||
      (rewrite fsubUset; destruct (IHt1 X), (IHt2 X)) ||
-     (rewrite fsub1set; destruct (s \in X) eqn:?));
+     (rewrite fsub1set; destruct (s ∈ X) eqn:?));
     constructor; intros_all; auto;
     inverts H; auto.
     rewrite /= Heqb // in H2.
   Qed.
 
-  Definition is_subset_of
-             (A B P__A P__B : Type)
-             `{HasMembers A P__A Prop}
-             `{HasMembers B P__B Prop}
-             (R : A -> B -> Prop)
-             (X : P__A)
-             (Y : P__B) :
-    Prop :=
-    forall a b, R a b -> (a ∈ X) /\ (b ∈ Y).
+  Definition is_subset_of R X Y : Prop :=
+    forall x y, R x y -> (x ∈ X) && (y ∈ Y).
 
   #[local] Notation "R '⊆' X '×' Y" := (is_subset_of R X Y) (at level 40, X at next level).
 
@@ -161,17 +151,17 @@ Module AlphaFacts (Import M : Alpha).
   (** Page 3: "R(x,y) ... ∈ (X ∪ {x}) × (Y ∪ {y})." *)
   Lemma update_type :
     forall X Y R x y,
-      (forall a b : 𝒱, R a b -> (a ∈ X : bool) : Prop /\ b ∈ Y) ->
-      (R : {fmap 𝒱 → 𝒱}) ⊆ X × Y ->
+      (forall a b : 𝒱, R a b -> a ∈ X /\ b ∈ Y) ->
+      R ⊆ X × Y ->
       R⦅x,y⦆ ⊆ (X ∪ {x}) × (Y ∪ {y}).
   Proof.
     unfold is_subset_of.
     intros.
     rewrite /= !in_fsetU !in_fset1.
     rewrite /fmap_to_Prop /update unionmE remmE setmE rem_valmE /= in H1.
-    destruct (a =P x); subst; inverts H1.
+    destruct (x0 =P x); subst; inverts H1.
     - rewrite eq_refl !orbT //.
-    - destruct (getm R a) eqn:?.
+    - destruct (getm R x0) eqn:?.
       + destruct (y =P s); subst; inverts H3.
         apply H in Heqo as []. simpl in *. rewrite H1 H2 //.
       + inverts H3.
@@ -195,7 +185,7 @@ Module AlphaFacts (Import M : Alpha).
 
     Inductive α_equivalent'' : {fmap 𝒱 -> 𝒱} -> term -> term -> Prop :=
     | α_equivalent''_variable : forall R x y,
-        (x, y) ∈ R : Prop ->
+        (x, y) ∈ R ->
         variable x ≡_α^R variable y
     | α_equivalent''_application : forall R t t' u u',
         t ≡_α^R t' -> u ≡_α^R u' ->
@@ -214,7 +204,7 @@ Module AlphaFacts (Import M : Alpha).
     intros.
     destruct (t ≡_α^R u) eqn:?; constructor.
     - gen R u. induction t; intros;
-      destruct u; inverts Heqb; auto;
+      destruct u; inverts Heqb; auto.
       apply (rwP andP) in H0 as []; auto.
     - intros_all.
       dependent induction H; inverts Heqb; auto.
@@ -226,40 +216,38 @@ Module AlphaFacts (Import M : Alpha).
   Lemma α_equivalent'_type :
     forall R t u,
       t ≡_α^R u ->
-      FV t ⊆ domm R /\ FV u ⊆ codomm R.
+      t ∈ Tm (domm R) /\ u ∈ Tm (codomm R).
   Proof.
+    rewrite /in_mem /= /Tm.
     intros_all.
     gen R u. induction t; simpl; intros;
     destruct u; inverts H;
     simpl in *.
-    - rewrite H1. apply IHt in H1 as [].
-      split; intros;
+    - apply IHt in H1 as []. apply (rwP fsubsetP) in H, H0.
+      split; apply (rwP fsubsetP); intros_all;
       rewrite in_fsetD in_fset1 in H1; apply (rwP andP) in H1 as []; apply negbTE in H1.
       + apply H, (rwP dommP) in H2 as [].
         rewrite unionmE remmE rem_valmE setmE H1 in H2.
-        destruct (getm R a) eqn:?; cycle 1.
+        destruct (getm R x) eqn:?; cycle 1.
         { inverts H2. }
         destruct (s0 =P s1); subst; inverts H2.
         apply (rwP dommP). eauto.
       + apply H0, (rwP codommP) in H2 as [].
         rewrite unionmE remmE rem_valmE setmE /= in H2.
-        destruct (x =P s); subst; auto.
+        destruct (x0 =P s); subst; auto.
         { inverts H2. rewrite eq_refl // in H1. }
-        destruct (getm R x) eqn:?; cycle 1.
+        destruct (getm R x0) eqn:?; cycle 1.
         { inverts H2. }
         destruct (s0 =P s1); subst; inverts H2.
         apply (rwP codommP). eauto.
     - apply (rwP andP) in H1 as [].
-      rewrite H H0.
       apply IHt1 in H as []. apply IHt2 in H0 as [].
-      split; intros; rewrite in_fsetU in H3; rewrite -H3.
-      destruct (a \in FV t1) eqn:?; destruct (a \in FV t2) eqn:?; auto.
-      { inverts H3. }
-      destruct (a \in FV u1) eqn:?; destruct (a \in FV u2) eqn:?; auto.
-      inverts H3.
-    - rewrite H1. apply (rwP eqP) in H1.
-      split; intros;
-      rewrite in_fset1 in H; apply (rwP eqP) in H; subst.
+      apply (rwP fsubsetP) in H, H0, H1, H2.
+      split; apply (rwP fsubsetP); intros_all;
+      rewrite in_fsetU in H3; apply (rwP orP) in H3 as []; auto.
+    - rewrite /in_mem /= /in_mem /= in H1. apply (rwP (getmP _ _ _)) in H1.
+      rewrite !fsub1set.
+      split.
       + apply (rwP dommP). eauto.
       + apply (rwP codommP). eauto.
   Qed.
@@ -288,7 +276,7 @@ Module AlphaFacts (Import M : Alpha).
   Proof.
     intros_all.
     rewrite /identity' /= /fmap_to_Prop mkfmapfE in H.
-    destruct (a \in X) eqn:?; rewrite Heqb0 // in H.
+    destruct (x ∈ X) eqn:?; rewrite Heqb in H;
     inverts H. auto.
   Qed.
 
@@ -302,8 +290,8 @@ Module AlphaFacts (Import M : Alpha).
     intros_all.
     apply (rwP dommP) in H as [].
     rewrite !mkfmapfE in H, H0.
-    destruct (x \in X) eqn:?; rewrite Heqb in H, H0; inverts H.
-    destruct (x2 \in X) eqn:?; rewrite Heqb0 in H0; inverts H0.
+    destruct (x ∈ X) eqn:?; rewrite Heqb in H, H0; inverts H.
+    destruct (x2 ∈ X) eqn:?; rewrite Heqb0 in H0; inverts H0.
     auto.
   Qed.
 
@@ -318,9 +306,8 @@ Module AlphaFacts (Import M : Alpha).
       R ⊆ X × Y ->
       R ᵒ ⊆ Y × X.
   Proof.
-    intros ? ? ? ?.
     intros_all.
-    rewrite /fmap_to_Prop in H0. apply getm_inv in H0. apply H in H0 as []. auto.
+    apply getm_inv, H in H0. rewrite andbC //.
   Qed.
 
   (** Page 3: "Both operations are closed under partial bijections." *)
@@ -357,9 +344,9 @@ Module AlphaFacts (Import M : Alpha).
   Proof.
     intros_all.
     rewrite /fmap_to_Prop mkfmapfpE in H1.
-    destruct (a \in domm R) eqn:?; rewrite Heqb0 // in H1.
-    apply (rwP dommP) in Heqb0 as []. rewrite H2 in H1.
-    apply H in H2 as []. apply H0 in H1 as []. auto.
+    destruct (x ∈ domm R) eqn:?; rewrite Heqb // in H1.
+    apply (rwP dommP) in Heqb as []. rewrite H2 in H1.
+    apply H, (rwP andP) in H2 as []. apply H0, (rwP andP) in H1 as []. rewrite H2 H4 //.
   Qed.
 
   (** Page 3: "Both operations are closed under partial bijections." *)
@@ -375,11 +362,11 @@ Module AlphaFacts (Import M : Alpha).
     simpl. rewrite <- (rwP (injectivemP _)). intros_all.
     apply (rwP dommP) in H1 as [].
     rewrite !mkfmapfpE in H1, H2.
-    destruct (x \in domm R) eqn:?; rewrite Heqb in H1, H2; cycle 1.
+    destruct (x ∈ domm R) eqn:?; rewrite Heqb in H1, H2; cycle 1.
     { inverts H1. }
     apply (rwP dommP) in Heqb as []. rewrite H3 in H1, H2.
     rewrite H1 in H2.
-    destruct (x2 \in domm R) eqn:?; rewrite Heqb in H2; cycle 1.
+    destruct (x2 ∈ domm R) eqn:?; rewrite Heqb in H2; cycle 1.
     { inverts H2. }
     apply (rwP dommP) in Heqb as []. rewrite H4 -H1 in H2.
     apply H0 in H2; cycle 1.
@@ -397,7 +384,7 @@ Module AlphaFacts (Import M : Alpha).
     rewrite unionmE mkfmapfE in_fsetU in_fset1 remmE rem_valmE /= setmE mkfmapfE.
     destruct (x0 =P x); subst.
     - rewrite orbT //.
-    - destruct (x0 \in X) eqn:?; rewrite Heqb.
+    - destruct (x0 ∈ X) eqn:?; rewrite Heqb.
       + replace (x == id x0) with false; auto.
         symmetry. apply Bool.not_true_iff_false. intros_all.
         apply (rwP eqP) in H. auto.
@@ -469,14 +456,14 @@ Module AlphaFacts (Import M : Alpha).
     destruct (k =P x); subst.
     - rewrite eq_refl /=. f_equal.
       rewrite mkfmapfpE in H.
-      destruct (x \in domm (R⦅x,y⦆)) eqn:?; rewrite Heqb // in H.
+      destruct (x ∈ domm (R⦅x,y⦆)) eqn:?; rewrite Heqb // in H.
       apply (rwP dommP) in Heqb as []. rewrite H0 in H.
       rewrite !unionmE !remmE !rem_valmE !setmE !eq_refl /= in H, H0.
       destruct (x0 =P y); subst; inverts H; auto.
       inverts H0. contradiction.
     - apply (introF eqP) in n. rewrite n mkfmapfpE.
       rewrite mkfmapfpE in H.
-      destruct (k \in domm (R⦅x,y⦆)) eqn:?; rewrite Heqb // in H.
+      destruct (k ∈ domm (R⦅x,y⦆)) eqn:?; rewrite Heqb // in H.
       apply (rwP dommP) in Heqb as [].
       rewrite unionmE remmE rem_valmE setmE /= n in H, H0.
       destruct (getm R k) eqn:?; rewrite ?Heqo in H, H0; cycle 1.
@@ -513,12 +500,12 @@ Module AlphaFacts (Import M : Alpha).
       apply IHt1 with (R__super := R__super) in H0; auto.
       apply IHt2 with (R__super := R__super) in H1; auto.
       rewrite /= H0 H1 //.
-    - apply (rwP eqP), H in H2. rewrite /= H2 //.
+    - apply (rwP (getmP _ _ _)), H in H2. apply (rwP (getmP _ _ _)). auto.
   Qed.
 
   Lemma α_equivalent'_with_behaviorally_identical_maps :
     forall R S t u,
-      (forall x y, R x y -> x ∈ free_variables t : Prop -> S x y) ->
+      (forall x y, R x y -> x ∈ FV t -> S x y) ->
       t ≡_α^R u ->
       t ≡_α^S u.
   Proof.
@@ -541,8 +528,8 @@ Module AlphaFacts (Import M : Alpha).
       intros;
       apply H; auto;
       rewrite /= in_fsetU H3 ?orbT //.
-    - apply (rwP eqP), H in H2.
-      + simpl in *. rewrite H2 //.
+    - apply (rwP (getmP _ _ _)), H in H2.
+      + simpl in *. apply (rwP (getmP _ _ _)). rewrite H2 //.
       + rewrite /= in_fset1 eq_refl //.
   Qed.
 
@@ -564,24 +551,25 @@ Module AlphaFacts (Import M : Alpha).
   (** Page 4: Proposition 2.1. *)
   Proposition α_equivalent'_identity :
     forall X t,
-      FV t ⊆ X ->
+      t ∈ Tm X ->
       t ≡_α^(1__X) t.
   Proof.
     intros.
+    apply (rwP fsubsetP) in H.
     gen X. induction t; intros; simpl.
     - rewrite update_identity.
-      apply IHt. simpl. intros.
+      apply IHt. simpl. intros_all.
       rewrite in_fsetU in_fset1 orbC.
-      destruct (a =P s); subst; auto.
+      destruct (x =P s); subst; auto.
       apply (introF eqP) in n.
       apply H. rewrite /= in_fsetD in_fset1 n H0 //.
     - rewrite <- (rwP andP). split;
       apply α_equivalent'_supermap with (R__sub := 1__X); auto; intros;
-      (apply IHt1 || apply IHt2); simpl; intros;
+      (apply IHt1 || apply IHt2); simpl; intros_all;
       apply H; rewrite /= in_fsetU H0 ?orbT //.
-    - assert (s \in fset1 s). { rewrite in_fset1 eq_refl //. }
+    - assert (s ∈ fset1 s). { rewrite in_fset1 eq_refl //. }
       apply H in H0. simpl in *.
-      rewrite mkfmapfE H0 //.
+      apply (rwP (getmP _ _ _)). rewrite mkfmapfE H0 //.
   Qed.
 
   (** Page 4: Proposition 2.2. *)
@@ -600,9 +588,9 @@ Module AlphaFacts (Import M : Alpha).
     - apply (rwP andP) in H2 as [].
       apply IHt1 in H0; auto. apply IHt2 in H1; auto.
       rewrite /= H0 H1 //.
-    - simpl. rewrite <- (rwP eqP). apply getm_inv. rewrite invmK.
-      + apply (rwP eqP). auto.
-      + apply (rwP (injectivemP _)). auto.
+    - apply (rwP (getmP _ _ _)) in H2.
+      apply (rwP (getmP _ _ _)), getm_inv. rewrite invmK //.
+      apply (rwP (injectivemP _)). auto.
   Qed.
 
   (** Page 4: Proposition 2.3. *)
@@ -623,17 +611,16 @@ Module AlphaFacts (Import M : Alpha).
       apply IHt1 with (R := R) (S := S) (v := v1) in H1; auto.
       apply IHt2 with (R := R) (S := S) (v := v2) in H2; auto.
       rewrite /= H1 H2 //.
-    - apply (rwP eqP) in H1, H2.
-      rewrite /= mkfmapfpE.
-      assert (exists s0, getm R s = Some s0) by eauto. apply (rwP dommP) in H. rewrite H H2.
-      rewrite <- (rwP eqP). auto.
+    - apply (rwP (getmP _ _ _)) in H1, H2.
+      apply (rwP (getmP _ _ _)). rewrite /= mkfmapfpE.
+      assert (exists s0, getm R s = Some s0) by eauto. apply (rwP dommP) in H. rewrite H H2 //.
   Qed.
 
-  Lemma α_equivalent'_maps_all_free_variables :
+  Lemma α_equivalent'_maps_all_FV :
     forall R t u x,
       t ≡_α^R u ->
-      x ∈ free_variables t : Prop ->
-      exists y, getm R x = Some y /\ y ∈ free_variables u.
+      x ∈ FV t ->
+      exists y, getm R x = Some y /\ y ∈ FV u.
   Proof.
     intros.
     gen R u. induction t; intros_all;
@@ -653,98 +640,100 @@ Module AlphaFacts (Import M : Alpha).
         exists x0. simpl in *. rewrite in_fsetU H2 //.
       + apply IHt2 with (u := u2) in H1 as (? & ? & ?); auto.
         exists x0. simpl in *. rewrite in_fsetU H2 orbT //.
-    - apply (rwP eqP) in H2.
+    - apply (rwP (getmP _ _ _)) in H2.
       rewrite /= in_fset1 in H0. apply (rwP eqP) in H0. subst.
       exists s0. rewrite /= in_fset1 eq_refl //.
   Qed.
 
-  Lemma α_equivalent'_maps_all_free_variables' :
+  Lemma α_equivalent'_maps_all_FV' :
     forall R t u y,
       partial_bijection R ->
       t ≡_α^R u ->
-      y ∈ free_variables u : Prop ->
-      exists x, getm R x = Some y /\ x ∈ free_variables t.
+      y ∈ FV u ->
+      exists x, getm R x = Some y /\ x ∈ FV t.
   Proof.
     intros.
     apply α_equivalent'_converse in H0; auto.
-    pose proof α_equivalent'_maps_all_free_variables _ _ _ H0 H1 as (? & ? & ?).
+    pose proof α_equivalent'_maps_all_FV _ _ _ _ H0 H1 as (? & ? & ?).
     apply getm_inv in H2. eauto.
   Qed.
 
-  Lemma α_equivalent'_implies_related_free_variables :
+  Lemma α_equivalent'_implies_related_FV :
     forall R t u,
       partial_bijection R ->
       t ≡_α^R u ->
-      free_variables u = pimfset (getm R) (free_variables t).
+      FV u = pimfset (getm R) (FV t).
   Proof.
     intros.
     apply eq_fset. intros_all.
     rewrite in_pimfset.
     symmetry.
-    destruct (x \in free_variables u) eqn:?.
-    - eapply α_equivalent'_maps_all_free_variables' in Heqb as (? & ? & ?); eauto.
+    destruct (x ∈ FV u) eqn:?.
+    - eapply α_equivalent'_maps_all_FV' in Heqb as (? & ? & ?); eauto.
       apply (rwP imfsetP). simpl in *. eauto.
     - apply Bool.not_true_iff_false. intros_all.
       apply (rwP imfsetP) in H1 as [].
-      eapply α_equivalent'_maps_all_free_variables in H1 as (? & ? & ?); eauto.
+      eapply α_equivalent'_maps_all_FV in H1 as (? & ? & ?); eauto.
       rewrite H1 in H2. inverts H2.
       simpl in *. rewrite H3 // in Heqb.
   Qed.
 
-  Lemma α_equivalent'_bijection_includes_all_free_variables :
+  Lemma α_equivalent'_bijection_includes_all_FV :
     forall R t u,
       t ≡_α^R u ->
-      free_variables t ⊆ domm R.
+      t ∈ Tm (domm R).
   Proof.
     intros.
+    rewrite /Tm /in_mem /=. apply (rwP fsubsetP).
     gen R u. induction t; intros_all;
     destruct u; inverts H.
     - rewrite /= in_fsetD in_fset1 in H0. apply (rwP andP) in H0 as [].
-      cut (a ∈ domm R⦅s,s0⦆ = true).
+      cut (x ∈ domm R⦅s,s0⦆ = true).
       { intros.
         simpl in *. apply (rwP dommP) in H1 as [].
         rewrite unionmE remmE rem_valmE setmE /= in H1.
-        destruct (a =P s); subst; auto.
-        destruct (getm R a) eqn:?.
+        destruct (x =P s); subst; auto.
+        destruct (getm R x) eqn:?.
         - eapply (rwP dommP). eauto.
         - inverts H1. }
       eapply IHt; eauto.
     - apply (rwP andP) in H2 as [].
       rewrite /= /in_mem /= in_fsetU in H0. apply (rwP orP) in H0 as [].
       apply IHt1 in H; auto. apply IHt2 in H1; auto.
-    - apply (rwP eqP) in H2. simpl in *. rewrite in_fset1 in H0. apply (rwP eqP) in H0. subst.
-      eapply (rwP dommP). eauto.
+    - apply (rwP (getmP _ _ _)) in H2.
+      simpl in *. rewrite in_fset1 in H0. apply (rwP eqP) in H0. subst.
+      apply (rwP dommP). eauto.
   Qed.
 
-  Lemma α_equivalent'_bijection_includes_all_free_variables' :
+  Lemma α_equivalent'_bijection_includes_all_FV' :
     forall R t u,
       partial_bijection R ->
       t ≡_α^R u ->
-      free_variables u ⊆ codomm R.
+      u ∈ Tm (codomm R).
   Proof.
     intros.
     eapply α_equivalent'_converse in H0; eauto.
     rewrite codomm_domm_invm //.
-    eapply α_equivalent'_bijection_includes_all_free_variables; eauto.
+    eapply α_equivalent'_bijection_includes_all_FV; eauto.
   Qed.
 
-  Lemma α_equivalent_implies_same_free_variables :
+  Lemma α_equivalent_implies_same_FV :
     forall t u,
       t ≡_α u ->
-      free_variables u = free_variables t.
+      FV u = FV t.
   Proof.
     intros.
-    replace (free_variables t) with (pimfset (getm (1__(free_variables t) : {fmap 𝒱 → 𝒱})) (free_variables t)); cycle 1.
+    replace (FV t) with (pimfset (getm (1__(FV t) : {fmap 𝒱 → 𝒱})) (FV t)); cycle 1.
     { apply eq_fset. intros_all.
       rewrite in_pimfset.
-      destruct (x \in free_variables t) eqn:?.
+      destruct (x ∈ FV t) eqn:?.
       - apply (rwP imfsetP).
         exists x; auto.
         rewrite mkfmapfE Heqb //.
       - apply negbTE, (introN imfsetP). intros [].
         rewrite mkfmapfE in H1.
         rewrite H0 in H1. inverts H1. rewrite H0 // in Heqb. }
-    eapply α_equivalent'_implies_related_free_variables; eauto.
+    eapply α_equivalent'_implies_related_FV; eauto.
     apply partial_bijection_identity.
   Qed.
 
@@ -752,7 +741,7 @@ Module AlphaFacts (Import M : Alpha).
   Proof.
     intros.
     apply eq_fset. intros_all.
-    destruct (x \in X) eqn:?.
+    destruct (x ∈ X) eqn:?.
     - apply (rwP dommP). exists x. rewrite mkfmapfE Heqb //.
     - apply negbTE. rewrite <- (rwP dommPn).
       rewrite mkfmapfE. rewrite Heqb //.
@@ -769,8 +758,8 @@ Module AlphaFacts (Import M : Alpha).
     simpl. intros.
     rewrite /fmap_to_Prop mkfmapfE in H.
     rewrite /fmap_to_Prop mkfmapfE H1.
-    eapply α_equivalent'_bijection_includes_all_free_variables in H1; eauto.
-    rewrite domm_identity /= in H1. rewrite H1 // in H.
+    eapply α_equivalent'_bijection_includes_all_FV in H0; eauto.
+    rewrite domm_identity /= in H0. apply (rwP fsubsetP) in H0. apply H0 in H1. rewrite H1 // in H.
   Qed.
 
   Lemma compose_identity_right : forall R, R; (1__(codomm R)) = R.
@@ -778,9 +767,9 @@ Module AlphaFacts (Import M : Alpha).
     intros.
     apply eq_fmap. intros_all.
     rewrite mkfmapfpE.
-    destruct (x \in domm R) eqn:?; rewrite Heqb.
+    destruct (x ∈ domm R) eqn:?; rewrite Heqb.
     - apply (rwP dommP) in Heqb as []. rewrite H mkfmapfE.
-      destruct (x0 \in codomm R) eqn:?; rewrite Heqb //.
+      destruct (x0 ∈ codomm R) eqn:?; rewrite Heqb //.
       apply negbT in Heqb.
       rewrite <- (rwP (@codommPn _ 𝒱 _ _)) in Heqb.
       pose proof Heqb x. rewrite H eq_refl // in H0.
@@ -792,7 +781,7 @@ Module AlphaFacts (Import M : Alpha).
     intros.
     apply eq_fmap. intros_all.
     rewrite mkfmapfpE mkfmapfE domm_mkfmapf in_fset.
-    destruct (x \in domm R) eqn:?; rewrite Heqb //.
+    destruct (x ∈ domm R) eqn:?; rewrite Heqb //.
     apply negbT, (rwP dommPn) in Heqb. auto.
   Qed.
 
@@ -800,12 +789,12 @@ Module AlphaFacts (Import M : Alpha).
   Proof.
     intros.
     apply eq_fset. intros_all.
-    destruct (x \in X) eqn:?.
+    destruct (x ∈ X) eqn:?.
     - apply (rwP codommP). exists x. rewrite mkfmapfE Heqb //.
     - apply negbTE. rewrite <- (rwP (@codommPn _ 𝒱 _ _)). intros_all.
       apply (introN eqP). intros_all.
       rewrite mkfmapfE in H.
-      destruct (k' \in X) eqn:?; rewrite Heqb0 in H; inverts H.
+      destruct (k' ∈ X) eqn:?; rewrite Heqb0 in H; inverts H.
       rewrite Heqb0 // in Heqb.
   Qed.
 
@@ -816,9 +805,9 @@ Module AlphaFacts (Import M : Alpha).
     intros.
     apply eq_fmap. intros_all.
     rewrite mkfmapfpE !mkfmapfE in_fsetI.
-    destruct (x \in X) eqn:?; rewrite Heqb;
+    destruct (x ∈ X) eqn:?; rewrite Heqb;
     rewrite domm_identity Heqb // mkfmapfE.
-    destruct (x \in Y) eqn:?; rewrite Heqb0 //.
+    destruct (x ∈ Y) eqn:?; rewrite Heqb0 //.
   Qed.
 
   Lemma compose_identity' : forall X, (1__X); (1__X) = 1__X.
@@ -833,7 +822,7 @@ Module AlphaFacts (Import M : Alpha).
     intros.
     apply eq_fmap. intros_all.
     rewrite mkfmapfE.
-    destruct (x \in X) eqn:?; rewrite Heqb.
+    destruct (x ∈ X) eqn:?; rewrite Heqb.
     - apply getm_inv. rewrite invmK.
       + rewrite mkfmapfE Heqb //.
       + apply (rwP (injectivemP _)). apply partial_bijection_identity.
@@ -842,14 +831,14 @@ Module AlphaFacts (Import M : Alpha).
       + rewrite <- (rwP (@codommPn _ 𝒱 _ _)). intros_all.
         apply (introN eqP). intros_all.
         rewrite mkfmapfE in H.
-        destruct (k' \in X) eqn:?; rewrite Heqb0 in H; inverts H.
+        destruct (k' ∈ X) eqn:?; rewrite Heqb0 in H; inverts H.
         rewrite Heqb0 // in Heqb.
   Qed.
 
   (** Page 4: "≡α is... reflexive." *)
   Corollary α_equivalent_reflexive : forall t, t ≡_α t.
   Proof.
-    intros. apply α_equivalent'_identity. auto.
+    intros. apply α_equivalent'_identity. rewrite /Tm /in_mem /= fsubsetxx //.
   Qed.
 
   (** Page 4: "≡α is... transitive." *)
@@ -866,8 +855,8 @@ Module AlphaFacts (Import M : Alpha).
     intros.
     rewrite mkfmapfE in_fsetI in H2.
     rewrite mkfmapfE.
-    destruct (k \in FV t) eqn:?; rewrite Heqb //.
-    destruct (k \in FV u) eqn:?; inverts H2. auto.
+    destruct (k ∈ FV t) eqn:?; rewrite Heqb //.
+    destruct (k ∈ FV u) eqn:?; inverts H2. auto.
   Qed.
 
   (** Page 4: "≡α is... symmetric." *)
@@ -902,23 +891,23 @@ Module AlphaFacts (Import M : Alpha).
 
   #[local] Notation "f '[' x ',' t ']'" := (update_substitution f x t) (at level 10, x at next level, t at next level).
 
-  Definition codomm_Tm_set f : {fset 𝒱} := ⋃_(i ∈ codomm f) (free_variables i).
+  Definition codomm_Tm_set f : {fset 𝒱} := ⋃_(i ∈ codomm f) (FV i).
 
   Lemma codomm_Tm_setP :
     forall {f} {x},
-      reflect (exists t, x ∈ free_variables t /\ t ∈ codomm f) (x ∈ codomm_Tm_set f).
+      reflect (exists t, x ∈ FV t /\ t ∈ codomm f) (x ∈ codomm_Tm_set f).
   Proof.
     intros.
     destruct (x ∈ codomm_Tm_set f) eqn:?; constructor;
-    rewrite /= /codomm_Tm_set in_bigcup in Heqy.
-    - apply (rwP hasP) in Heqy as []. exists x0. auto.
-    - apply negbT, (rwP hasPn) in Heqy. intros (? & ? & ?).
-      apply Heqy in H0. simpl in *. rewrite H // in H0.
+    rewrite /= /codomm_Tm_set in_bigcup in Heqb.
+    - apply (rwP hasP) in Heqb as []. exists x0. auto.
+    - apply negbT, (rwP hasPn) in Heqb. intros (? & ? & ?).
+      apply Heqb in H0. simpl in *. rewrite H // in H0.
   Qed.
 
   #[local] Reserved Notation "'⦇' f '⦈'".
 
-  (** Page 4: "A substitution can be extended to a function on terms ⦇f⦈ \in Tm(X) ⟶ Tm(Y)...." *)
+  (** Page 4: "A substitution can be extended to a function on terms ⦇f⦈ ∈ Tm(X) ⟶ Tm(Y)...." *)
   Fixpoint lift_substitution f t : term :=
     match t with
     | variable x => odflt t (getm f x)
@@ -969,12 +958,12 @@ Module AlphaFacts (Import M : Alpha).
     - destruct (getm R z) eqn:?; cycle 1.
       { inverts H2. }
       destruct (y =P s); subst; inverts H2.
-      assert (z \in domm R) by (apply (rwP dommP); eauto). rewrite H2 // in H.
+      assert (z ∈ domm R) by (apply (rwP dommP); eauto). rewrite H2 // in H.
     - destruct (getm R k) eqn:?; cycle 1.
       { inverts H2. }
       destruct (y =P s); subst; inverts H2.
       destruct (z' =P v); subst.
-      { assert (v \in codomm R) by (apply (rwP codommP); eauto). rewrite H2 // in H0. }
+      { assert (v ∈ codomm R) by (apply (rwP codommP); eauto). rewrite H2 // in H0. }
       apply (introF eqP) in n1. rewrite /= n1 //.
   Qed.
 
@@ -982,18 +971,18 @@ Module AlphaFacts (Import M : Alpha).
     forall R x y z z',
       z ∉ domm R ->
       z' ∉ codomm R ->
-      (x, y) ∈ R : Prop ->
-      (x, y) ∈ R⦅z,z'⦆ : Prop.
+      (x, y) ∈ R ->
+      (x, y) ∈ R⦅z,z'⦆.
   Proof.
     intros.
     simpl in *.
-    apply (rwP eqP) in H1.
-    apply (rwP (@eqP _ _ (Some y))).
+    apply (rwP (getmP _ _ _)) in H1.
+    apply (rwP (getmP _ _ _)).
     rewrite /update unionmE remmE rem_valmE setmE /= H1.
     destruct (x =P z); subst.
-    { assert (z \in domm R) by (apply (rwP dommP); eauto). rewrite H2 // in H. }
+    { assert (z ∈ domm R) by (apply (rwP dommP); eauto). rewrite H2 // in H. }
     destruct (z' =P y); subst; auto.
-    assert (y \in codomm R) by (apply (rwP codommP); eauto). rewrite H2 // in H0.
+    assert (y ∈ codomm R) by (apply (rwP codommP); eauto). rewrite H2 // in H0.
   Qed.
 
   Lemma update_repeat_noop :
@@ -1011,7 +1000,7 @@ Module AlphaFacts (Import M : Alpha).
 
   Lemma codomm_Tm_setPn :
     forall {f} {x},
-      reflect (forall t, ~ (x ∈ free_variables t /\ t ∈ codomm f)) (x ∉ codomm_Tm_set f).
+      reflect (forall t, ~ (x ∈ FV t /\ t ∈ codomm f)) (x ∉ codomm_Tm_set f).
   Proof.
     intros.
     destruct (x ∉ codomm_Tm_set f) eqn:?;
@@ -1026,7 +1015,7 @@ Module AlphaFacts (Import M : Alpha).
 
   Lemma α_equivalent'_with_behaviorally_identical_maps' :
     forall R S t u,
-      (forall x y, R x y -> x ∈ free_variables t : Prop -> y ∈ free_variables u : Prop -> S x y) ->
+      (forall x y, R x y -> x ∈ FV t -> y ∈ FV u -> S x y) ->
       t ≡_α^R u ->
       t ≡_α^S u.
   Proof.
@@ -1050,8 +1039,8 @@ Module AlphaFacts (Import M : Alpha).
       intros;
       apply H; auto;
       rewrite /= in_fsetU ?H3 ?H4 ?orbT //.
-    - apply (rwP eqP), H in H2.
-      + simpl in *. rewrite H2 //.
+    - apply (rwP (getmP _ _ _)), H in H2.
+      + simpl in *. apply (rwP (getmP _ _ _)). rewrite H2 //.
       + rewrite /= in_fset1 eq_refl //.
       + rewrite /= in_fset1 eq_refl //.
   Qed.
@@ -1074,13 +1063,14 @@ Module AlphaFacts (Import M : Alpha).
     destruct (w =P x); subst.
     - inverts H5.
       rewrite !eq_refl.
+      apply (rwP (getmP _ _ _)).
       rewrite /= unionmE remmE rem_valmE eq_refl setmE eq_refl //.
     - destruct (getm R w) eqn:?; cycle 1.
       { inverts H5. }
       destruct (y =P s); subst; inverts H5.
       apply not_eq_sym, (introF eqP) in n0. rewrite n0.
       pose proof Heqo. apply H2 in Heqo. inverts Heqo.
-      apply H in H5 as [].
+      apply H, (rwP andP) in H5 as [].
       simpl in *. apply (rwP dommP) in H5 as [], H6 as [].
       rewrite -> H5, H6 in *. simpl in *.
       apply α_equivalent'_with_behaviorally_identical_maps' with (R := S); auto. intros.
@@ -1098,13 +1088,14 @@ Module AlphaFacts (Import M : Alpha).
 
   Lemma subset_domm_substitution :
     forall f x t,
-      domm f ⊆ domm (f[x,t]).
+      fsubset (domm f) (domm (f[x,t])).
   Proof.
-    simpl. intros.
+    intros.
+    apply (rwP fsubsetP). intros_all.
     apply (rwP dommP) in H as [].
     apply (rwP dommP).
     rewrite setmE.
-    destruct (a =P x); subst; eauto.
+    destruct (x0 =P x); subst; eauto.
   Qed.
 
   (** Page 4: Proposition 4. *)
@@ -1125,27 +1116,27 @@ Module AlphaFacts (Import M : Alpha).
       + rewrite !domm_set /=. intros_all.
         rewrite /= !in_fsetU !in_fset1.
         rewrite /fmap_to_Prop unionmE remmE rem_valmE setmE /= in H3.
-        destruct (a =P s); subst.
+        destruct (x =P s); subst.
         { inverts H3. rewrite eq_refl //. }
-        destruct (getm R a) eqn:?; cycle 1.
+        destruct (getm R x) eqn:?; cycle 1.
         { inverts H3. }
         destruct (s0 =P s1); subst; inverts H3.
-        apply H in Heqo as []. simpl in *. rewrite H3 H4 orbT //.
+        apply H, (rwP andP) in Heqo as []. simpl in *. rewrite H3 H4 orbT //.
       + intros. eapply lemma5; eauto; apply Fresh_correct.
     - apply (rwP andP) in H5 as [].
       eapply IHt1 with (S := S) in H3; eauto.
       eapply IHt2 with (S := S) in H4; eauto.
       rewrite /= H3 H4 //.
-    - apply (rwP eqP) in H5. simpl in *.
+    - apply (rwP (getmP _ _ _)) in H5. simpl in *.
       pose proof H5. apply H2 in H3.
-      apply H in H5 as [].
+      apply H, (rwP andP) in H5 as [].
       simpl in *. apply (rwP dommP) in H4 as [], H5 as [].
       rewrite -> H4, H5 in *. auto.
   Qed.
 
   #[program] Corollary substitution_preserves_α_congruence_identity :
     forall f g,
-      (forall x, x ∈ domm f ∩ domm g : Prop -> getm f x `≡_α^(1__(codomm_Tm_set f ∩ codomm_Tm_set g)) getm g x) ->
+      (forall x, x ∈ domm f ∩ domm g -> getm f x `≡_α^(1__(codomm_Tm_set f ∩ codomm_Tm_set g)) getm g x) ->
       forall t u, t ≡_α^(1__(domm f ∩ domm g)) u -> ⦇f⦈ t ≡_α^(1__(codomm_Tm_set f ∩ codomm_Tm_set g)) ⦇g⦈ u.
   Proof.
     intros.
@@ -1153,56 +1144,56 @@ Module AlphaFacts (Import M : Alpha).
     try apply partial_bijection_identity.
     - simpl. intros_all.
       rewrite /fmap_to_Prop mkfmapfE in_fsetI in H1.
-      destruct (a \in domm f) eqn:?; inverts H1.
-      destruct (a \in domm g) eqn:?; inverts H3.
-      rewrite /= Heqb1 //.
+      destruct (x ∈ domm f) eqn:?; inverts H1.
+      destruct (x ∈ domm g) eqn:?; inverts H3.
+      rewrite /= Heqb0 //.
     - intros.
       rewrite /= /identity /fmap_to_Prop mkfmapfE in_fsetI in H1.
-      destruct (x \in domm f) eqn:?; inverts H1.
-      destruct (x \in domm g) eqn:?; inverts H3.
+      destruct (x ∈ domm f) eqn:?; inverts H1.
+      destruct (x ∈ domm g) eqn:?; inverts H3.
       apply H. rewrite /= in_fsetI Heqb Heqb0 //.
   Qed.
 
   (** Page 5: "Clearly, the preservation property arises as a special case by setting R = 1X and S = 1Y." *)
   #[program] Theorem substitution_preserves_α_congruence :
     forall f g,
-      (forall x, x ∈ domm f ∩ domm g : Prop -> getm f x `≡_α getm g x) ->
-      forall t u, FV t ⊆ (domm f ∩ domm g) -> t ≡_α u -> ⦇f⦈ t ≡_α ⦇g⦈ u.
+      (forall x, x ∈ domm f ∩ domm g -> getm f x `≡_α getm g x) ->
+      forall t u, t ∈ Tm (domm f ∩ domm g) -> t ≡_α u -> ⦇f⦈ t ≡_α ⦇g⦈ u.
   Proof.
     intros.
     eapply α_equivalent'_implies_α_equivalent. exists (codomm_Tm_set f ∩ codomm_Tm_set g).
     apply substitution_preserves_α_congruence_identity.
     - simpl. intros.
       rewrite in_fsetI in H2. apply (rwP andP) in H2 as [].
-      assert (x \in domm f ∩ domm g). { rewrite in_fsetI H2 H3 //. }
+      assert (x ∈ domm f ∩ domm g). { rewrite in_fsetI H2 H3 //. }
       apply H in H4.
       apply (rwP dommP) in H2 as [], H3 as [].
       rewrite H2 H3 /=. rewrite H2 H3 /= in H4.
       apply α_equivalent'_supermap with (R__sub := 1__(FV x0)); auto.
       intros.
       rewrite mkfmapfE in H5.
-      destruct (k \in FV x0) eqn:?; rewrite Heqb in H5; inverts H5.
+      destruct (k ∈ FV x0) eqn:?; rewrite Heqb in H5; inverts H5.
       rewrite mkfmapfE in_fsetI.
-      assert (v \in codomm_Tm_set f).
+      assert (v ∈ codomm_Tm_set f).
       { apply (rwP codomm_Tm_setP). exists x0. split; auto.
         simpl. apply (rwP codommP). eauto. }
-      assert (v \in codomm_Tm_set g).
+      assert (v ∈ codomm_Tm_set g).
       { apply (rwP codomm_Tm_setP). exists x1.
-        apply α_equivalent_implies_same_free_variables in H4.
+        apply α_equivalent_implies_same_FV in H4.
         rewrite H4. split; auto.
         simpl. apply (rwP codommP). eauto. }
       rewrite H5 H6 //.
     - apply α_equivalent'_supermap with (R__sub := 1__(FV t)); auto.
       intros.
       rewrite mkfmapfE in H2.
-      destruct (k \in FV t) eqn:?; rewrite Heqb in H2; inverts H2.
-      simpl in *. apply H0 in Heqb. rewrite mkfmapfE Heqb //.
+      destruct (k ∈ FV t) eqn:?; rewrite Heqb in H2; inverts H2.
+      simpl in *. apply (rwP fsubsetP) in H0. apply H0 in Heqb. rewrite mkfmapfE Heqb //.
   Qed.
 
   (** Page 5: "A consequence of proposition 4 is that substitution is an operation on α-equivalence classes." *)
   Theorem substitution_respects_α_equivalence :
     forall f t u,
-      FV t ⊆ domm f ->
+      t ∈ Tm (domm f) ->
       t ≡_α u ->
       ⦇f⦈ t ≡_α ⦇f⦈ u.
   Proof.
@@ -1235,10 +1226,11 @@ Module AlphaFacts (Import M : Alpha).
   Lemma lemma7 :
     forall (f : {fmap 𝒱 → 𝒱}) t,
       partial_bijection f ->
-      FV t ⊆ domm f ->
+      t ∈ Tm (domm f) ->
       ⦇mapm variable f⦈ t ≡_α^(f ᵒ) t.
   Proof.
     intros.
+    apply (rwP fsubsetP) in H0.
     gen f. induction t; intros; simpl in *.
     - rewrite /= /update_substitution -mapm_setm -/update_substitution -update_converse //.
       rewrite codomm_Tm_set_mapm_variable.
@@ -1248,30 +1240,30 @@ Module AlphaFacts (Import M : Alpha).
         destruct (x =P s); subst; auto.
         destruct (getm f x) eqn:?; auto.
         destruct (Fresh (codomm f) =P s0); subst; auto.
-        assert (Fresh (codomm f) \in codomm f). { apply (rwP codommP). eauto. }
+        assert (Fresh (codomm f) ∈ codomm f). { apply (rwP codommP). eauto. }
         pose proof Fresh_correct (codomm f). rewrite H1 // in H2. }
       apply IHt; auto.
       + apply partial_bijection_update. auto.
-      + intros.
+      + intros_all.
         apply (rwP dommP).
         rewrite unionmE remmE rem_valmE setmE /=.
-        destruct (a =P s); subst; simpl; eauto.
-        assert (a \in FV t :\ s).
+        destruct (x =P s); subst; simpl; eauto.
+        assert (x ∈ FV t :\ s).
         { apply (introF eqP) in n. rewrite in_fsetD in_fset1 n H1 //. }
         apply H0, (rwP dommP) in H2 as []. rewrite H2 /=.
-        destruct (Fresh (codomm f) =P x); subst; simpl; eauto.
-        assert (Fresh (codomm f) \in codomm f). { apply (rwP codommP). eauto. }
+        destruct (Fresh (codomm f) =P x0); subst; simpl; eauto.
+        assert (Fresh (codomm f) ∈ codomm f). { apply (rwP codommP). eauto. }
         pose proof Fresh_correct (codomm f). rewrite H3 // in H4.
     - rewrite <- (rwP andP). split.
-      + apply IHt1; auto. intros.
+      + apply IHt1; auto. intros_all.
         apply H0. rewrite in_fsetU H1 //.
-      + apply IHt2; auto. intros.
+      + apply IHt2; auto. intros_all.
         apply H0. rewrite in_fsetU H1 orbT //.
     - apply α_equivalent'_converse; auto.
       rewrite /= mapmE.
-      assert (s \in fset1 s). { rewrite in_fset1 eq_refl //. }
+      assert (s ∈ fset1 s). { rewrite in_fset1 eq_refl //. }
       apply H0, (rwP dommP) in H1 as [].
-      rewrite H1 /= eq_refl //.
+      rewrite H1 /=. apply (rwP (getmP _ _ _)). auto.
   Qed.
 
   (** Page 6: "η(x) = x." *)
@@ -1289,7 +1281,7 @@ Module AlphaFacts (Import M : Alpha).
     - apply (rwP codomm_Tm_setP) in H as (? & ? & ?).
       simpl in *. apply (rwP codommP) in H0 as [].
       rewrite mapmE mkfmapfE in H0.
-      destruct (x1 \in X) eqn:?; rewrite Heqb in H0; inverts H0.
+      destruct (x1 ∈ X) eqn:?; rewrite Heqb in H0; inverts H0.
       rewrite in_fset1 in H. apply (rwP eqP) in H. subst. auto.
     - apply (rwP codomm_Tm_setP). exists (variable x). split.
       { rewrite /= in_fset1 eq_refl //. }
@@ -1359,12 +1351,13 @@ Module AlphaFacts (Import M : Alpha).
       + rewrite H. eauto.
   Qed.
 
-  Lemma free_variables_lift_substitution :
+  Lemma FV_lift_substitution :
     forall f t,
-      FV t ⊆ domm f ->
+      t ∈ Tm (domm f) ->
       FV (⦇f⦈ t) = ⋃_(u ∈ pimfset (getm f) (FV t)) (FV u).
   Proof.
     intros.
+    apply (rwP fsubsetP) in H.
     apply eq_fset. intros_all.
     rewrite in_bigcup.
     apply Bool.eq_iff_eq_true.
@@ -1381,25 +1374,25 @@ Module AlphaFacts (Import M : Alpha).
           apply (rwP (pimfsetP _ _ _)). exists x1; auto.
           apply (introF eqP) in n.
           rewrite in_fsetD in_fset1 n H1 //.
-        * intros.
+        * intros_all.
           rewrite domm_update_substitution in_fsetU in_fset1 orbC.
-          destruct (a =P s); subst; auto.
+          destruct (x0 =P s); subst; auto.
           apply (introF eqP) in n.
           apply H. rewrite in_fsetD in_fset1 n H2 //.
       + rewrite in_fsetU in H0. apply (rwP orP) in H0 as [].
         * apply IHt1 in H0 as []; cycle 1.
-          { intros. apply H. rewrite in_fsetU H1 //. }
+          { intros_all. apply H. rewrite in_fsetU H1 //. }
           apply (rwP (pimfsetP _ _ _)) in H0 as [].
           exists x0; auto.
           apply (rwP (pimfsetP _ _ _)). exists x1; auto.
           rewrite in_fsetU H0 //.
         * apply IHt2 in H0 as []; cycle 1.
-          { intros. apply H. rewrite in_fsetU H1 orbT //. }
+          { intros_all. apply H. rewrite in_fsetU H1 orbT //. }
           apply (rwP (pimfsetP _ _ _)) in H0 as [].
           exists x0; auto.
           apply (rwP (pimfsetP _ _ _)). exists x1; auto.
           rewrite in_fsetU H0 orbT //.
-      + assert (s \in fset1 s). { rewrite in_fset1 eq_refl //. }
+      + assert (s ∈ fset1 s). { rewrite in_fset1 eq_refl //. }
         apply H, (rwP dommP) in H1 as [].
         exists x0.
         * apply (rwP (pimfsetP (getm f) (fset1 s) x0)). exists s; auto.
@@ -1410,15 +1403,15 @@ Module AlphaFacts (Import M : Alpha).
       gen f. induction t; intros; simpl in *.
       + rewrite in_fsetD in_fset1 in H0. apply (rwP andP) in H0 as [].
         rewrite in_fsetD in_fset1.
-        assert (x \in codomm_Tm_set f).
+        assert (x ∈ codomm_Tm_set f).
         { apply (rwP codomm_Tm_setP). exists x0. split; auto. simpl. apply (rwP codommP). eauto. }
         pose proof Fresh_correct (codomm_Tm_set f).
         destruct (x =P Fresh (codomm_Tm_set f)); subst.
         { rewrite H4 // in H5. }
         apply IHt; auto.
-        * intros.
+        * intros_all.
           rewrite domm_set in_fsetU in_fset1.
-          destruct (a =P s); subst; auto.
+          destruct (x2 =P s); subst; auto.
           apply (introF eqP) in n0.
           apply H.
           rewrite in_fsetD in_fset1 n0 H6 //.
@@ -1428,10 +1421,10 @@ Module AlphaFacts (Import M : Alpha).
         apply (rwP orP) in H0 as [].
         * eapply IHt1 in H0; eauto.
           -- rewrite H0 //.
-          -- intros. apply H. rewrite in_fsetU H3 //.
+          -- intros_all. apply H. rewrite in_fsetU H3 //.
         * eapply IHt2 in H0; eauto.
           -- rewrite H0 orbT //.
-          -- intros. apply H. rewrite in_fsetU H3 orbT //.
+          -- intros_all. apply H. rewrite in_fsetU H3 orbT //.
       + rewrite in_fset1 in H0. apply (rwP eqP) in H0. subst.
         rewrite H2 //.
   Qed.
@@ -1439,12 +1432,12 @@ Module AlphaFacts (Import M : Alpha).
   (** Page 4: "⦇f⦈ ∈ Tm(X) ⟶ Tm(Y)." *)
   Lemma lift_substitution_type :
     forall f t,
-      t ∈ Tm (domm f) : Prop -> ⦇f⦈ t ∈ Tm (codomm_Tm_set f) : Prop.
+      t ∈ Tm (domm f) ->
+      ⦇f⦈ t ∈ Tm (codomm_Tm_set f).
   Proof.
     intros.
-    apply (rwP fsubsetP) in H.
-    rewrite /= /Tm. apply (rwP fsubsetP). intros_all.
-    rewrite free_variables_lift_substitution // in_bigcup in H0. apply (rwP hasP) in H0 as [].
+    rewrite /Tm /in_mem /=. apply (rwP fsubsetP). intros_all.
+    rewrite FV_lift_substitution // in_bigcup in H0. apply (rwP hasP) in H0 as [].
     apply (rwP (pimfsetP _ _ _)) in H0 as [].
     apply (rwP codomm_Tm_setP). exists x0. split; auto.
     simpl. apply (rwP codommP). eauto.
@@ -1452,24 +1445,25 @@ Module AlphaFacts (Import M : Alpha).
 
   #[program] Lemma lift_substitution_indistinguishable_substitutions' :
     forall R f g t,
-      FV t ⊆ (domm f ∩ domm g) ->
-      (forall x, x ∈ FV t : Prop -> getm f x `≡_α^R getm g x) ->
+      t ∈ Tm (domm f ∩ domm g) ->
+      (forall x, x ∈ FV t -> getm f x `≡_α^R getm g x) ->
       ⦇f⦈ t ≡_α^R ⦇g⦈ t.
   Proof.
     intros.
+    apply (rwP fsubsetP) in H.
     gen R f g. induction t; intros.
-    - apply IHt; simpl; intros.
+    - apply IHt; simpl; intros_all.
       + rewrite in_fsetI !domm_set !in_fsetU !in_fset1.
-        destruct (a =P s); subst; auto.
+        destruct (x =P s); subst; auto.
         apply (introF eqP) in n.
-        assert (a \in FV t :\ s). { rewrite in_fsetD in_fset1 n H1 //. }
+        assert (x ∈ FV t :\ s). { rewrite in_fsetD in_fset1 n H1 //. }
         apply H in H2. rewrite /= in_fsetI in H2. apply (rwP andP) in H2 as [].
         rewrite H2 H3 //.
       + rewrite !setmE.
         destruct (x =P s); subst.
-        { rewrite /= unionmE remmE rem_valmE setmE eq_refl //. }
+        { apply (rwP (getmP _ _ _)). rewrite /= unionmE remmE rem_valmE setmE eq_refl //. }
         apply (introF eqP) in n.
-        assert (x \in FV t :\ s). { rewrite in_fsetD in_fset1 n H1 //. }
+        assert (x ∈ FV t :\ s). { rewrite in_fsetD in_fset1 n H1 //. }
         apply α_equivalent_update'; eauto;
         apply negbT, Bool.not_true_iff_false; intros_all; simpl in *;
         apply H in H2; rewrite in_fsetI in H2; apply (rwP andP) in H2 as [];
@@ -1479,20 +1473,21 @@ Module AlphaFacts (Import M : Alpha).
         * apply (H5 x0). split; auto. simpl. apply (rwP codommP). eauto.
         * apply (H6 x1). split; auto. simpl. apply (rwP codommP). eauto.
     - simpl. rewrite <- (rwP andP). split;
-      (apply IHt1 || apply IHt2); simpl; intros;
+      (apply IHt1 || apply IHt2); simpl; intros_all;
       (apply H || apply H0); rewrite /= in_fsetU H1 ?orbT //.
     - apply H0. rewrite /= in_fset1 eq_refl //.
   Qed.
 
   #[program] Lemma lift_substitution_indistinguishable_substitutions :
     forall f g t,
-      FV t ⊆ (domm f ∩ domm g) ->
-      (forall x, x ∈ FV t : Prop -> getm f x `≡_α getm g x) ->
+      t ∈ Tm (domm f ∩ domm g) ->
+      (forall x, x ∈ FV t -> getm f x `≡_α getm g x) ->
       ⦇f⦈ t ≡_α ⦇g⦈ t.
   Proof.
     intros.
     apply lift_substitution_indistinguishable_substitutions'; auto.
     simpl. intros.
+    apply (rwP fsubsetP) in H.
     do 2 pose proof H1. apply H0 in H1.
     apply H in H2. rewrite /= in_fsetI in H2. apply (rwP andP) in H2 as [].
     apply (rwP dommP) in H2 as [].
@@ -1500,11 +1495,12 @@ Module AlphaFacts (Import M : Alpha).
     { apply H1. }
     intros.
     rewrite mkfmapfE H2 in H5. inverts H5.
-    destruct (k \in FV x0) eqn:?; rewrite Heqb in H7; inverts H7.
+    destruct (k ∈ FV x0) eqn:?; rewrite Heqb in H7; inverts H7.
     rewrite mkfmapfE Heqb.
-    cut (v \in FV (⦇f⦈ t) : Prop). { intros. rewrite H5 //. }
-    rewrite free_variables_lift_substitution; cycle 1.
-    { simpl. intros. apply H in H5. rewrite /= in_fsetI in H5. apply (rwP andP) in H5 as []. auto. }
+    cut (v ∈ FV (⦇f⦈ t) : Prop). { intros. rewrite H5 //. }
+    rewrite FV_lift_substitution; cycle 1.
+    { rewrite /Tm /in_mem /=. apply (rwP fsubsetP). intros_all.
+      apply H in H5. rewrite /= in_fsetI in H5. apply (rwP andP) in H5 as []. auto. }
     rewrite in_bigcup. apply (rwP hasP). exists x0; auto.
     apply (rwP (pimfsetP _ _ _)). eauto.
   Qed.
@@ -1512,12 +1508,13 @@ Module AlphaFacts (Import M : Alpha).
   (** Page 7: "We have to show ⦇f[[z0 = z1]]⦈ ∘ g[[x = z0]](v) ≡α (⦇f⦈ ∘ g)[[x = z1]](v)." *)
   #[program] Lemma lift_update_substitution_compose_substitution_update :
     forall f g x z0 z1,
-      codomm_Tm_set g ⊆ domm f ->
+      fsubset (codomm_Tm_set g) (domm f) ->
       z1 ∉ codomm_Tm_set f ->
       z0 ∉ codomm_Tm_set g ->
-      forall v, v \in (domm g ∪ {x}) -> getm (⦇f[z0,variable z1]⦈ ∘ g[x,variable z0]) v `≡_α getm ((⦇f⦈ ∘ g)[x,variable z1]) v.
+      forall v, v ∈ (domm g ∪ {x}) -> getm (⦇f[z0,variable z1]⦈ ∘ g[x,variable z0]) v `≡_α getm ((⦇f⦈ ∘ g)[x,variable z1]) v.
   Proof.
     intros.
+    apply (rwP fsubsetP) in H.
     rewrite !setmE !mapmE /= !setmE.
     rewrite in_fsetU in_fset1 in H2. apply (rwP orP) in H2 as []; cycle 1.
     { rewrite H2 /= setmE eq_refl. reflexivity. }
@@ -1525,34 +1522,37 @@ Module AlphaFacts (Import M : Alpha).
     { rewrite /= setmE eq_refl. reflexivity. }
     apply (rwP dommP) in H2 as []. rewrite H2 /=.
     apply lift_substitution_indistinguishable_substitutions; simpl; intros.
-    - rewrite domm_set in_fsetI in_fsetU in_fset1 orbC.
-      destruct (a \in domm f) eqn:?; auto.
-      assert (a \in codomm_Tm_set g).
+    - rewrite /Tm /in_mem /=. apply (rwP fsubsetP). intros_all.
+      rewrite domm_set in_fsetI in_fsetU in_fset1 orbC.
+      destruct (x1 ∈ domm f) eqn:?; auto.
+      assert (x1 ∈ codomm_Tm_set g).
       { apply (rwP codomm_Tm_setP). exists x0. split; auto. simpl. apply (rwP codommP). eauto. }
       apply H in H4. rewrite /= Heqb // in H4.
     - rewrite setmE.
       destruct (x1 =P z0); subst.
-      + assert (z0 \in codomm_Tm_set g).
+      + assert (z0 ∈ codomm_Tm_set g).
         { apply (rwP codomm_Tm_setP). exists x0. split; auto. simpl. apply (rwP codommP). eauto. }
         rewrite H4 // in H1.
       + reflexivity.
   Qed.
 
-  Lemma free_variables_lift_substitution_η :
+  Lemma FV_lift_substitution_η :
     forall X t,
-      FV t ⊆ X ->
+      t ∈ Tm X ->
       FV (⦇η__ X⦈ t) = FV t.
   Proof.
     intros.
-    rewrite free_variables_lift_substitution; cycle 1.
-    { simpl. intros. rewrite domm_map domm_mkfmapf in_fset. apply H. auto. }
+    apply (rwP fsubsetP) in H.
+    rewrite FV_lift_substitution; cycle 1.
+    { rewrite /Tm /in_mem /=. apply (rwP fsubsetP). intros_all.
+      rewrite domm_map domm_mkfmapf in_fset. apply H. auto. }
     apply eq_fset. intros_all.
     rewrite in_bigcup.
     apply Bool.eq_iff_eq_true. split; intros.
     - apply (rwP hasP) in H0 as [].
       apply (rwP (pimfsetP _ _ _)) in H0 as [].
       rewrite mapmE mkfmapfE in H2.
-      destruct (x1 \in X) eqn:?; rewrite Heqb in H2; inverts H2.
+      destruct (x1 ∈ X) eqn:?; rewrite Heqb in H2; inverts H2.
       rewrite in_fset1 in H1. apply (rwP eqP) in H1. subst. auto.
     - apply (rwP hasP). exists (variable x).
       + apply (rwP (pimfsetP _ _ _)). exists x; auto.
@@ -1563,24 +1563,27 @@ Module AlphaFacts (Import M : Alpha).
 
   Proposition monad_substitution1 :
     forall X t,
-      FV t ⊆ X ->
+      t ∈ Tm X ->
       ⦇η__ X⦈ t ≡_α t.
   Proof.
     intros.
+    apply (rwP fsubsetP) in H.
     transitivity (⦇η__(FV t)⦈ t).
     { apply lift_substitution_indistinguishable_substitutions; simpl; intros.
-      - rewrite in_fsetI !domm_map domm_mkfmapf domm_mkfmapf !in_fset H0 andbT. apply H. auto.
+      - rewrite /Tm /in_mem /=. apply (rwP fsubsetP). intros_all.
+        rewrite in_fsetI !domm_map domm_mkfmapf domm_mkfmapf !in_fset H0 andbT. auto.
       - rewrite !mapmE !mkfmapfE H0. apply H in H0. simpl in *. rewrite H0. reflexivity. }
     rewrite /α_equivalent -converse_identity.
-    rewrite free_variables_lift_substitution_η //.
+    rewrite FV_lift_substitution_η //.
     apply lemma7.
     - apply partial_bijection_identity.
-    - simpl. intros. rewrite domm_mkfmapf in_fset H0 //.
+    - rewrite /Tm /in_mem /=. apply (rwP fsubsetP). intros_all. rewrite domm_mkfmapf in_fset H0 //.
+    - rewrite /Tm /in_mem /=. apply (rwP fsubsetP). intros_all. auto.
   Qed.
 
   #[program] Proposition monad_substitution2 :
     forall f x,
-      x ∈ domm f : Prop ->
+      x ∈ domm f ->
       getm (⦇f⦈ ∘ η__(domm f)) x `≡_α getm f x.
   Proof.
     simpl. intros. rewrite !mapmE mkfmapfE H. reflexivity.
@@ -1588,10 +1591,11 @@ Module AlphaFacts (Import M : Alpha).
 
   #[program] Lemma codomm_Tm_set_mapm :
     forall f g,
-      codomm_Tm_set g ⊆ domm f ->
+      fsubset (codomm_Tm_set g) (domm f) ->
       codomm_Tm_set (mapm ⦇f⦈ g) = ⋃_(x ∈ codomm_Tm_set g) (FV (odflt (variable _) (getm f x))).
   Proof.
     intros.
+    apply (rwP fsubsetP) in H.
     apply eq_fset. intros_all.
     rewrite in_bigcup.
     apply Bool.eq_iff_eq_true. split; intros.
@@ -1599,8 +1603,8 @@ Module AlphaFacts (Import M : Alpha).
       simpl in *. apply (rwP codommP) in H1 as [].
       rewrite mapmE in H1.
       destruct (getm g x1) eqn:?; inverts H1.
-      rewrite free_variables_lift_substitution in H0; cycle 1.
-      { simpl. intros.
+      rewrite FV_lift_substitution in H0; cycle 1.
+      { rewrite /Tm /in_mem /=. apply (rwP fsubsetP). intros_all.
         apply H, (rwP codomm_Tm_setP). exists t. split; auto. simpl. apply (rwP codommP). eauto. }
       rewrite in_bigcup in H0. apply (rwP hasP) in H0 as [].
       apply (rwP (pimfsetP _ _ _)) in H0 as [].
@@ -1614,8 +1618,8 @@ Module AlphaFacts (Import M : Alpha).
       apply (rwP codomm_Tm_setP) in H2 as (? & ? & ?).
       simpl in *. apply (rwP codommP) in H3 as [].
       apply (rwP codomm_Tm_setP). exists (⦇f⦈ x2). split.
-      { rewrite free_variables_lift_substitution; cycle 1.
-        { simpl. intros.
+      { rewrite FV_lift_substitution; cycle 1.
+        { rewrite /Tm /in_mem /=. apply (rwP fsubsetP). intros_all.
           apply H, (rwP codomm_Tm_setP). exists x2. split; auto. simpl. apply (rwP codommP). eauto. }
         rewrite /= in_bigcup. apply (rwP hasP). exists x1; auto.
         apply (rwP (pimfsetP _ _ _)). exists x0; auto. }
@@ -1625,11 +1629,12 @@ Module AlphaFacts (Import M : Alpha).
 
   Proposition monad_substitution3 :
     forall f g t,
-      codomm_Tm_set g ⊆ domm f ->
-      FV t ⊆ domm g ->
+      fsubset (codomm_Tm_set g) (domm f) ->
+      t ∈ Tm (domm g) ->
       (⦇f⦈ ∘ ⦇g⦈) t ≡_α ⦇⦇f⦈ ∘ g⦈ t.
   Proof.
     intros.
+    apply (rwP fsubsetP) in H, H0.
     gen f g. induction t; intros.
     - set (z0 := Fresh (codomm_Tm_set g)).
       set (z1 := Fresh (codomm_Tm_set f)).
@@ -1639,89 +1644,96 @@ Module AlphaFacts (Import M : Alpha).
         rewrite mkfmapfE in H1.
         rewrite mkfmapfE in_fsetU in_fsetD !in_fset1 orbC.
         destruct (k =P z1); subst; auto.
-        destruct (z1 \in X) eqn:?; rewrite Heqb in H1; inverts H1. auto. }
+        destruct (z1 ∈ X) eqn:?; rewrite Heqb in H1; inverts H1. auto. }
       transitivity (⦇f⦈ (abstraction z0 (⦇g[s,variable z0]⦈ t))).
       { rewrite /α_equivalent/= update_identity -/z0 -/z1 -/X.
         apply α_equivalent'_supermap with (R__sub := 1__X); auto.
-        apply α_equivalent'_identity. auto. }
+        apply α_equivalent'_identity.
+        rewrite /Tm /in_mem /=. apply (rwP fsubsetP). intros_all. auto. }
       transitivity (abstraction z1 ((⦇f[z0,variable z1]⦈ ∘ ⦇g[s,variable z0]⦈) t)).
       { rewrite /α_equivalent /= update_identity -/z0 -/z1 -/X.
         apply α_equivalent'_supermap with (R__sub := 1__X); auto.
-        apply α_equivalent'_identity. auto. }
+        apply α_equivalent'_identity.
+        rewrite /Tm /in_mem /=. apply (rwP fsubsetP). intros_all. auto. }
       assert (⦇f[z0,variable z1]⦈ (⦇g[s,variable z0]⦈ t) ≡_α ⦇⦇f[z0,variable z1]⦈ ∘ g[s,variable z0]⦈ t).
-      { apply IHt; simpl; intros;
+      { apply IHt; simpl; intros_all;
         rewrite domm_set in_fsetU in_fset1.
-        - destruct (a =P z0); subst; auto.
+        - destruct (x =P z0); subst; auto.
           apply (rwP codomm_Tm_setP) in H2 as (? & ? & ?).
           simpl in *. apply (rwP codommP) in H3 as [].
           rewrite setmE in H3.
-          destruct (x0 =P s); subst.
+          destruct (x1 =P s); subst.
           { inverts H3. rewrite in_fset1 in H2. apply (rwP eqP) in H2. subst. contradiction. }
-          apply H, (rwP codomm_Tm_setP). exists x. split; auto.
+          apply H, (rwP codomm_Tm_setP). exists x0. split; auto.
           simpl. apply (rwP codommP). eauto.
-        - destruct (a =P s); subst; auto.
+        - destruct (x =P s); subst; auto.
           apply (introF eqP) in n.
           apply H0. rewrite /= in_fsetD in_fset1 n H2 //. }
       transitivity (abstraction z1 (⦇⦇f[z0,variable z1]⦈ ∘ g[s,variable z0]⦈ t)).
       { rewrite /α_equivalent /= update_identity -/z0 -/z1 -/X.
         apply α_equivalent'_supermap with (R__sub := 1__X); auto. }
       transitivity (abstraction z1 (⦇(⦇f⦈ ∘ g)[s,variable z1]⦈ t)).
-      { apply α_equivalent_implies_same_free_variables in H2.
+      { apply α_equivalent_implies_same_FV in H2.
         rewrite /α_equivalent /= update_identity -/z0 -/z1 H2 -/X.
         apply α_equivalent'_supermap with (R__sub := 1__X); auto.
         rewrite /X -H2.
         apply lift_substitution_indistinguishable_substitutions; simpl; intros.
-        - rewrite in_fsetI domm_set !domm_map domm_set !in_fsetU in_fset1 Bool.andb_diag.
-          destruct (a =P s); subst; auto.
+        - rewrite /Tm /in_mem /=. apply (rwP fsubsetP). intros_all.
+          rewrite in_fsetI domm_set !domm_map domm_set !in_fsetU in_fset1 Bool.andb_diag.
+          destruct (x =P s); subst; auto.
           apply (introF eqP) in n.
           apply H0. rewrite /= in_fsetD in_fset1 n H3 //.
         - apply lift_update_substitution_compose_substitution_update; auto; try apply Fresh_correct.
-          rewrite in_fsetU in_fset1 orbC.
-          destruct (x =P s); subst; auto.
-          apply (introF eqP) in n.
-          apply H0. rewrite /= in_fsetD in_fset1 n H3 //. }
+          + apply (rwP fsubsetP). auto.
+          + rewrite in_fsetU in_fset1 orbC.
+            destruct (x =P s); subst; auto.
+            apply (introF eqP) in n.
+            apply H0. rewrite /= in_fsetD in_fset1 n H3 //. }
       rewrite /α_equivalent /=.
       apply substitution_preserves_α_congruence' with (R := 1__(FV t)).
-      { rewrite !domm_set !domm_map.
-        split; intros;
+      { rewrite !domm_set !domm_map. intros_all.
+        rewrite <- (rwP andP).
+        split;
         rewrite /= !in_fsetU !in_fset1;
         rewrite /fmap_to_Prop mkfmapfE in H3;
-        destruct (a \in FV t) eqn:?; rewrite Heqb0 in H3; inverts H3;
-        destruct (b =P s); subst; auto;
+        destruct (x ∈ FV t) eqn:?; rewrite Heqb in H3; inverts H3;
+        destruct (y =P s); subst; auto;
         apply (introF eqP) in n;
-        simpl in *; apply H0; rewrite /= in_fsetD in_fset1 n Heqb0 //. }
+        simpl in *; apply H0; rewrite /= in_fsetD in_fset1 n Heqb //. }
       { apply partial_bijection_identity. }
       { apply partial_bijection_update, partial_bijection_identity. }
       { intros.
         rewrite /fmap_to_Prop mkfmapfE in H3.
-        destruct (x \in FV t) eqn:?; rewrite Heqb in H3; inverts H3.
+        destruct (x ∈ FV t) eqn:?; rewrite Heqb in H3; inverts H3.
         rewrite !setmE !mapmE.
         destruct (x' =P s); subst.
-        { rewrite /= unionmE remmE rem_valmE setmE eq_refl //. }
+        { apply (rwP (getmP _ _ _)). rewrite /= unionmE remmE rem_valmE setmE eq_refl //. }
         apply (introF eqP) in n.
         simpl in *.
-        assert (x' \in FV t :\ s). { rewrite in_fsetD in_fset1 n Heqb //. }
+        assert (x' ∈ FV t :\ s). { rewrite in_fsetD in_fset1 n Heqb //. }
         apply H0, (rwP dommP) in H3 as []. rewrite H3 /=.
-        assert (FV x ⊆ codomm_Tm_set g).
-        { simpl. intros. apply (rwP codomm_Tm_setP). exists x. split; auto. simpl. apply (rwP codommP). eauto. }
-        assert (FV (⦇f⦈ x) ⊆ codomm_Tm_set (mapm ⦇f⦈ g)).
-        { simpl. intros.
-          rewrite free_variables_lift_substitution in H5; cycle 1.
-          { simpl. intros. apply H, H4, H5. }
+        assert {subset FV x <= codomm_Tm_set g}.
+        { intros_all. apply (rwP codomm_Tm_setP). exists x. split; auto. simpl. apply (rwP codommP). eauto. }
+        assert {subset FV (⦇f⦈ x) <= codomm_Tm_set (mapm ⦇f⦈ g)}.
+        { intros_all.
+          rewrite FV_lift_substitution in H5; cycle 1.
+          { rewrite /Tm /in_mem /=. apply (rwP fsubsetP). intros_all. apply H, H4, H5. }
           rewrite in_bigcup in H5. apply (rwP hasP) in H5 as [].
           apply (rwP (pimfsetP _ _ _)) in H5 as [].
-          rewrite /= codomm_Tm_set_mapm // in_bigcup.
-          apply (rwP hasP). exists x1.
+          rewrite /= codomm_Tm_set_mapm; cycle 1.
+          { apply (rwP fsubsetP). intros_all. auto. }
+          rewrite in_bigcup.
+          apply (rwP hasP). exists x2.
           { apply H4. auto. }
           rewrite /= H7 //. }
-        assert (FV (⦇f⦈ x) ⊆ codomm_Tm_set f).
-        { simpl. intros.
-          rewrite free_variables_lift_substitution in H6; cycle 1.
-          { simpl. intros.
+        assert {subset FV (⦇f⦈ x) <= codomm_Tm_set f}.
+        { intros_all.
+          rewrite FV_lift_substitution in H6; cycle 1.
+          { rewrite /Tm /in_mem /=. apply (rwP fsubsetP). intros_all.
             apply H, (rwP codomm_Tm_setP). exists x. split; auto. simpl. apply (rwP codommP). eauto. }
           rewrite in_bigcup in H6. apply (rwP hasP) in H6 as [].
           apply (rwP (pimfsetP _ _ _)) in H6 as [].
-          apply (rwP codomm_Tm_setP). exists x0. split; auto. simpl. apply (rwP codommP). eauto. }
+          apply (rwP codomm_Tm_setP). exists x1. split; auto. simpl. apply (rwP codommP). eauto. }
         assert (Fresh (codomm_Tm_set (mapm ⦇f⦈ g)) ∉ FV (⦇f⦈ x)).
         { pose proof Fresh_correct (codomm_Tm_set (mapm ⦇f⦈ g)).
           apply negbT, Bool.not_true_iff_false. intros_all.
@@ -1737,43 +1749,44 @@ Module AlphaFacts (Import M : Alpha).
         intros.
         rewrite mkfmapfE in H9.
         rewrite mkfmapfE in_fsetD in_fset1.
-        destruct (k \in FV (⦇f⦈ x)) eqn:?; rewrite Heqb0 in H9; inverts H9.
+        destruct (k ∈ FV (⦇f⦈ x)) eqn:?; rewrite Heqb0 in H9; inverts H9.
         destruct (v =P z1); subst.
         { rewrite Heqb0 // in H8. }
-        rewrite free_variables_lift_substitution; cycle 1.
-        { simpl. intros.
+        rewrite FV_lift_substitution; cycle 1.
+        { rewrite /Tm /in_mem /=. apply (rwP fsubsetP). intros_all.
           rewrite domm_set domm_map in_fsetU in_fset1.
-          destruct (a =P s); subst; auto.
+          destruct (x0 =P s); subst; auto.
           apply (introF eqP) in n1.
           apply H0. rewrite in_fsetD in_fset1 n1 H9 //. }
         rewrite in_bigcup /=.
-        cut (has (fun i => v \in FV i)
+        cut (has (fun i => v ∈ FV i)
                   (pimfset (getm ((mapm ⦇f⦈ g)[s,variable z1])) (FV t)) : Prop).
         { intros. rewrite H9 //. }
         apply (rwP hasP). exists (⦇f⦈ x); auto.
         rewrite <- (rwP (pimfsetP (getm ((mapm ⦇f⦈ g)[s,variable z1])) (FV t) (⦇f⦈ x))).
         exists x'; auto.
         rewrite setmE mapmE n H3 //. }
-      apply α_equivalent'_identity. auto.
+      apply α_equivalent'_identity.
+      rewrite /Tm /in_mem /=. apply (rwP fsubsetP). intros_all. auto.
     - rewrite /α_equivalent /=. rewrite <- (rwP andP). split.
       + apply α_equivalent'_supermap with (R__sub := 1__(FV (⦇f⦈ (⦇g⦈ t1)))); cycle 1.
-        { apply IHt1; auto. simpl in *. intros. apply H0. rewrite in_fsetU H1 //. }
+        { apply IHt1; auto. simpl in *. intros_all. apply H0. rewrite in_fsetU H1 //. }
         intros.
         rewrite mkfmapfE in H1.
-        destruct (k \in FV (⦇f⦈ (⦇g⦈ t1))) eqn:?; rewrite Heqb in H1; inverts H1.
+        destruct (k ∈ FV (⦇f⦈ (⦇g⦈ t1))) eqn:?; rewrite Heqb in H1; inverts H1.
         rewrite mkfmapfE in_fsetU Heqb //.
       + apply α_equivalent'_supermap with (R__sub := 1__(FV (⦇f⦈ (⦇g⦈ t2)))); cycle 1.
-        { apply IHt2; auto. simpl in *. intros. apply H0. rewrite in_fsetU H1 orbT //. }
+        { apply IHt2; auto. simpl in *. intros_all. apply H0. rewrite in_fsetU H1 orbT //. }
         intros.
         rewrite mkfmapfE in H1.
-        destruct (k \in FV (⦇f⦈ (⦇g⦈ t2))) eqn:?; rewrite Heqb in H1; inverts H1.
+        destruct (k ∈ FV (⦇f⦈ (⦇g⦈ t2))) eqn:?; rewrite Heqb in H1; inverts H1.
         rewrite mkfmapfE in_fsetU Heqb orbT //.
     - simpl in *.
-      assert (s \in fset1 s). { rewrite in_fset1 //. }
+      assert (s ∈ fset1 s). { rewrite in_fset1 //. }
       apply H0, (rwP dommP) in H1 as []. rewrite mapmE H1. reflexivity.
   Qed.
 
-  Notation "t '[' x '=' u ']'" := (⦇(1__(free_variables t))[x,u]⦈ t) (at level 10, x at next level, u at next level).
+  Notation "t '[' x '=' u ']'" := (⦇(1__(FV t))[x,u]⦈ t) (at level 10, x at next level, u at next level).
 
   #[local] Notation "t '[' x '⟵' u ']'" := (t[x=u]) (at level 10, x at next level, u at next level).
 
@@ -1786,12 +1799,14 @@ Module AlphaFacts (Import M : Alpha).
     intros.
     transitivity (⦇η__(FV t)⦈ t).
     - apply lift_substitution_indistinguishable_substitutions; simpl; intros.
-      + rewrite !domm_map !domm_set !domm_map !domm_mkfmapf in_fsetI in_fsetU !in_fset H0 orbT //.
+      + rewrite /Tm /in_mem /=. apply (rwP fsubsetP). intros_all.
+        rewrite !domm_map !domm_set !domm_map !domm_mkfmapf in_fsetI in_fsetU !in_fset H0 orbT //.
       + rewrite setmE mapmE.
         destruct (x0 =P x); subst.
         { rewrite H0 // in H. }
         reflexivity.
-    - apply monad_substitution1. auto.
+    - apply monad_substitution1.
+      rewrite /Tm /in_mem /= fsubsetxx //.
   Qed.
 
   Lemma codomm_update_substitution :
@@ -1846,16 +1861,16 @@ Module AlphaFacts (Import M : Alpha).
     - apply (rwP codommP) in H as [].
       rewrite mapmE mkfmapfE in H.
       apply (rwP imfsetP).
-      destruct (x0 \in X) eqn:?; rewrite Heqb in H; inverts H.
+      destruct (x0 ∈ X) eqn:?; rewrite Heqb in H; inverts H.
       eauto.
     - apply (rwP imfsetP) in H as []. subst.
       apply (rwP codommP). exists x0.
       rewrite mapmE mkfmapfE H //.
   Qed.
 
-  Lemma free_variables_after_substitute :
+  Lemma FV_after_substitute :
     forall t u x,
-      x ∈ FV t : Prop ->
+      x ∈ FV t ->
       FV (t[x⟵u]) = (FV t :\ x) ∪ FV u.
   Proof.
     intros.
@@ -1869,9 +1884,9 @@ Module AlphaFacts (Import M : Alpha).
         rewrite remmE mapmE mkfmapfE in H1.
         destruct (x0 =P x); subst.
         { inverts H1. }
-        destruct (x0 \in FV t) eqn:?; rewrite Heqb in H1; inverts H1.
+        destruct (x0 ∈ FV t) eqn:?; rewrite Heqb in H1; inverts H1.
         rewrite in_fset1 in H0. apply (rwP eqP) in H0. subst. auto.
-      - destruct (x0 \in FV t) eqn:?.
+      - destruct (x0 ∈ FV t) eqn:?.
         + apply (rwP codomm_Tm_setP). exists (variable x0). simpl. split.
           * rewrite in_fset1 eq_refl //.
           * apply (rwP codommP). exists x0.
@@ -1882,9 +1897,9 @@ Module AlphaFacts (Import M : Alpha).
           rewrite remmE mapmE mkfmapfE in H1.
           destruct (x1 =P x); subst.
           { inverts H1. }
-          destruct (x1 \in FV t) eqn:?; rewrite Heqb0 in H1; inverts H1.
+          destruct (x1 ∈ FV t) eqn:?; rewrite Heqb0 in H1; inverts H1.
           rewrite in_fset1 in H0. apply (rwP eqP) in H0. subst. rewrite Heqb0 // in Heqb. }
-    rewrite free_variables_lift_substitution.
+    rewrite FV_lift_substitution.
     - apply eq_fset. intros_all.
       apply Bool.eq_iff_eq_true. split; simpl; intros.
       + rewrite in_fsetU.
@@ -1908,7 +1923,7 @@ Module AlphaFacts (Import M : Alpha).
           rewrite remmE mapmE mkfmapfE in H1.
           destruct (x2 =P x); subst.
           { inverts H1. }
-          destruct (x2 \in FV t) eqn:?; rewrite Heqb in H1; inverts H1.
+          destruct (x2 ∈ FV t) eqn:?; rewrite Heqb in H1; inverts H1.
           rewrite in_fset1 in H0. apply (rwP eqP) in H0. subst.
           exists (variable x2).
           -- apply (rwP (pimfsetP _ _ _)). exists x2; auto.
@@ -1918,17 +1933,17 @@ Module AlphaFacts (Import M : Alpha).
         * exists u; auto.
           apply (rwP (pimfsetP _ _ _)). exists x; auto.
           rewrite setmE mapmE mkfmapfE eq_refl //.
-    - simpl. intros.
+    - rewrite /Tm /in_mem /=. apply (rwP fsubsetP). intros_all.
       rewrite domm_set domm_map domm_mkfmapf in_fsetU in_fset H0 orbT //.
   Qed.
 
-  Lemma free_variables_noop_substitute :
+  Lemma FV_noop_substitute :
     forall t u x,
-      x ∉ FV t : Prop ->
+      x ∉ FV t ->
       FV (t[x⟵u]) = FV t.
   Proof.
     intros.
-    apply α_equivalent_implies_same_free_variables.
+    apply α_equivalent_implies_same_FV.
     symmetry. apply substitution_law1. auto.
   Qed.
 
@@ -1954,7 +1969,7 @@ Module AlphaFacts (Import M : Alpha).
       rewrite remmE mapmE mkfmapfE in H0.
       destruct (x2 =P x); subst.
       { inverts H0. }
-      destruct (x2 \in X) eqn:?; rewrite Heqb in H0; inverts H0.
+      destruct (x2 ∈ X) eqn:?; rewrite Heqb in H0; inverts H0.
       rewrite in_fset1 in H. apply (rwP eqP) in H. subst.
       apply (introF eqP) in n.
       rewrite n Heqb //.
@@ -1977,110 +1992,117 @@ Module AlphaFacts (Import M : Alpha).
     symmetry.
     transitivity (⦇⦇(1__(FV(⦇(1__(FV t))[y,v]⦈ t)))[x,⦇(1__(FV u))[y,v]⦈ u]⦈ ∘ (1__(FV t))[y,v]⦈ t).
     { destruct (y ∈ FV t) eqn:?. (* TODO Can we remove the [destruct]s of this form? *)
-      - apply monad_substitution3; simpl; intros; rewrite domm_set domm_map domm_mkfmapf in_fsetU in_fset.
-        + rewrite free_variables_after_substitute // in_fsetU in_fsetD !in_fset1.
-          destruct (a =P x); subst; auto.
+      - apply monad_substitution3; try rewrite /Tm /in_mem /=; apply (rwP fsubsetP); intros_all;
+        rewrite domm_set domm_map domm_mkfmapf in_fsetU in_fset.
+        + rewrite FV_after_substitute // in_fsetU in_fsetD !in_fset1.
+          destruct (x0 =P x); subst; auto.
           apply (rwP codomm_Tm_setP) in H1 as (? & ? & ?).
           simpl in *. apply (rwP codommP) in H2 as [].
           rewrite setmE mapmE mkfmapfE in H2.
-          destruct (x1 =P y); subst.
+          destruct (x2 =P y); subst.
           { inverts H2. rewrite H1 orbT //. }
           apply (introF eqP) in n0.
-          destruct (x1 \in FV t) eqn:?; rewrite Heqb in H2; inverts H2.
+          destruct (x2 ∈ FV t) eqn:?; rewrite Heqb0 in H2; inverts H2.
           rewrite in_fset1 in H1. apply (rwP eqP) in H1. subst.
-          rewrite n0 Heqb //.
+          rewrite n0 Heqb0 //.
         + rewrite H1 orbT //.
       - transitivity (⦇(1__(FV(⦇(1__(FV t))[y,v]⦈ t)))[x,⦇(1__(FV u))[y,v]⦈ u]⦈ t).
         { apply substitution_respects_α_equivalence.
-          - simpl. intros.
+          - rewrite /Tm /in_mem /=. apply (rwP fsubsetP). intros_all.
             rewrite domm_set domm_map domm_mkfmapf in_fsetU in_fset H1 orbT //.
-          - apply substitution_law1. simpl in *. rewrite Heqy0 //. }
+          - apply substitution_law1. simpl in *. rewrite Heqb //. }
         apply lift_substitution_indistinguishable_substitutions; simpl; intros.
-        + rewrite !domm_set !domm_map !domm_set !domm_map !domm_mkfmapf in_fsetI !in_fsetU !in_fset !in_fset1 H1 orbT andbT.
-          destruct (a =P x); subst; auto.
-          rewrite free_variables_noop_substitute //. simpl in *. rewrite Heqy0 //.
+        + rewrite /Tm /in_mem /=. apply (rwP fsubsetP). intros_all.
+          rewrite !domm_set !domm_map !domm_set !domm_map !domm_mkfmapf in_fsetI !in_fsetU !in_fset !in_fset1 H1 orbT andbT.
+          destruct (x0 =P x); subst; auto.
+          rewrite FV_noop_substitute //. simpl in *. rewrite Heqb //.
         + rewrite !setmE !mapmE !setmE !mapmE !mkfmapfE H1.
           destruct (x0 =P x); subst.
           { apply (introF eqP) in H. rewrite /= H /= setmE mapmE eq_refl. reflexivity. }
           apply (introF eqP) in n.
-          rewrite free_variables_noop_substitute; cycle 1.
-          { simpl in *. rewrite Heqy0 //. }
+          rewrite FV_noop_substitute; cycle 1.
+          { simpl in *. rewrite Heqb //. }
           rewrite H1 /=.
           destruct (x0 =P y); subst.
-          { rewrite /= H1 // in Heqy0. }
+          { rewrite /= H1 // in Heqb. }
           rewrite /= setmE mapmE mkfmapfE n H1. reflexivity. }
     symmetry.
     transitivity (⦇⦇(1__(FV (⦇(1__(FV t))[x,u]⦈ t)))[y,v]⦈ ∘ (1__(FV t))[x,u]⦈ t).
     { destruct (x ∈ FV t) eqn:?.
-      - apply monad_substitution3; simpl; intros; rewrite domm_set domm_map domm_mkfmapf in_fsetU in_fset1 in_fset.
-        + rewrite free_variables_after_substitute // in_fsetU in_fsetD !in_fset1.
-          destruct (a =P y); subst; auto.
+      - apply monad_substitution3; try rewrite /Tm /in_mem /=; apply (rwP fsubsetP); intros_all; rewrite domm_set domm_map domm_mkfmapf in_fsetU in_fset1 in_fset.
+        + rewrite FV_after_substitute // in_fsetU in_fsetD !in_fset1.
+          destruct (x0 =P y); subst; auto.
           apply (rwP codomm_Tm_setP) in H1 as (? & ? & ?).
           simpl in *. apply (rwP codommP) in H2 as [].
           rewrite setmE mapmE mkfmapfE in H2.
-          destruct (x1 =P x); subst.
-          { inverts H2. rewrite H1 orbT //. }
+          destruct (x2 =P x); subst.
+          { inverts H2. rewrite H1 !orbT //. }
           apply (introF eqP) in n0.
-          destruct (x1 \in FV t) eqn:?; rewrite Heqb in H2; inverts H2.
+          destruct (x2 ∈ FV t) eqn:?; rewrite Heqb0 in H2; inverts H2.
           rewrite in_fset1 in H1. apply (rwP eqP) in H1. subst.
-          rewrite n0 Heqb //.
+          rewrite n0 Heqb0 //.
         + rewrite H1 orbT //.
       - transitivity (⦇(1__(FV (⦇(1__(FV t))[x,u]⦈ t)))[y,v]⦈ t).
         { apply substitution_respects_α_equivalence; cycle 1.
-          { apply substitution_law1. simpl in *. rewrite Heqy0 //. }
-          simpl. intros.
+          { apply substitution_law1. simpl in *. rewrite Heqb //. }
+          rewrite /Tm /in_mem /=. apply (rwP fsubsetP). intros_all.
           rewrite domm_set domm_map domm_mkfmapf in_fsetU in_fset in_fset1 H1 orbT //. }
         apply lift_substitution_indistinguishable_substitutions; simpl; intros.
-        + rewrite !domm_set !domm_map !domm_set !domm_map !domm_mkfmapf in_fsetI !in_fsetU !in_fset !in_fset1 H1 orbT andbT free_variables_noop_substitute; cycle 1.
-          { simpl in *. rewrite Heqy0 //. }
-          destruct (a =P y); subst; auto.
+        + rewrite /Tm /in_mem /=. apply (rwP fsubsetP). intros_all.
+          rewrite !domm_set !domm_map !domm_set !domm_map !domm_mkfmapf in_fsetI !in_fsetU !in_fset !in_fset1 H1 orbT andbT FV_noop_substitute; cycle 1.
+          { simpl in *. rewrite Heqb //. }
+          destruct (x0 =P y); subst; auto.
         + rewrite !mapmE !setmE !mapmE !mkfmapfE H1.
           destruct (x0 =P y); subst.
           { apply not_eq_sym, (introF eqP) in H. rewrite H /= setmE eq_refl. reflexivity. }
           apply (introF eqP) in n.
           destruct (x0 =P x); subst.
-          { rewrite /= H1 // in Heqy0. }
-          rewrite /= setmE mapmE mkfmapfE n free_variables_noop_substitute; cycle 1.
-          { simpl in *. rewrite Heqy0 //. }
+          { rewrite /= H1 // in Heqb. }
+          rewrite /= setmE mapmE mkfmapfE n FV_noop_substitute; cycle 1.
+          { simpl in *. rewrite Heqb //. }
           rewrite H1. reflexivity. }
     apply lift_substitution_indistinguishable_substitutions; simpl; intros.
-    - rewrite !domm_map !domm_set !domm_map !domm_mkfmapf in_fsetI !in_fsetU !in_fset !in_fset1 H1 !orbT //.
+    - rewrite /Tm /in_mem /=. apply (rwP fsubsetP). intros_all.
+      rewrite !domm_map !domm_set !domm_map !domm_mkfmapf in_fsetI !in_fsetU !in_fset !in_fset1 H1 !orbT //.
     - rewrite !mapmE !setmE !mapmE !mkfmapfE H1.
       destruct (x0 =P x); subst.
       + apply (introF eqP) in H. rewrite H /= setmE mapmE mkfmapfE eq_refl /=.
         apply lift_substitution_indistinguishable_substitutions; simpl; intros.
-        * rewrite domm_set domm_map domm_set domm_map !domm_mkfmapf in_fsetI !in_fsetU !in_fset1 !in_fset H2 orbT andbT.
-          destruct (a =P y); subst; auto.
-          rewrite /= free_variables_after_substitute // in_fsetU in_fsetD !in_fset1 H2 orbT //.
+        * rewrite /Tm /in_mem /=. apply (rwP fsubsetP). intros_all.
+          rewrite domm_set domm_map domm_set domm_map !domm_mkfmapf in_fsetI !in_fsetU !in_fset1 !in_fset H2 orbT andbT.
+          destruct (x =P y); subst; auto.
+          rewrite /= FV_after_substitute // in_fsetU in_fsetD !in_fset1 H2 !orbT //.
         * rewrite !setmE !mapmE !mkfmapfE H2.
           destruct (x0 =P y); subst.
           { reflexivity. }
-          rewrite free_variables_after_substitute // in_fsetU in_fsetD !in_fset1 H2 orbT. reflexivity.
+          rewrite FV_after_substitute // in_fsetU in_fsetD !in_fset1 H2 orbT. reflexivity.
       + destruct (x0 =P y); subst.
-        * rewrite /= setmE mapmE eq_refl free_variables_after_substitute //.
+        * rewrite /= setmE mapmE eq_refl FV_after_substitute //.
           transitivity (⦇1__(FV v)⦈ v).
-          { symmetry. apply monad_substitution1. auto. }
+          { symmetry. apply monad_substitution1.
+            rewrite /Tm /in_mem /=. apply (rwP fsubsetP). intros_all. auto. }
           apply lift_substitution_indistinguishable_substitutions; simpl; intros.
-          -- rewrite domm_set !domm_map !domm_mkfmapf in_fsetI in_fsetU in_fset in_fset in_fsetU in_fsetD !in_fset1 H2 !orbT //.
+          -- rewrite /Tm /in_mem /=. apply (rwP fsubsetP). intros_all.
+             rewrite domm_set !domm_map !domm_mkfmapf in_fsetI in_fsetU in_fset in_fset in_fsetU in_fsetD !in_fset1 H2 !orbT //.
           -- rewrite setmE !mapmE !mkfmapfE in_fsetU in_fsetD in_fset1 H2 orbT.
              destruct (x0 =P x); subst.
              { rewrite H2 // in H0. }
              reflexivity.
         * apply (introF eqP) in n, n0.
           rewrite /= !setmE !mapmE !mkfmapfE n n0.
-          destruct (x \in FV t) eqn:?.
-          -- rewrite free_variables_after_substitute // in_fsetU in_fsetD in_fset1 H1 andbT n /=.
-             destruct (y \in FV t) eqn:?.
-             ++ rewrite free_variables_after_substitute // in_fsetU in_fsetD in_fset1 H1 n0. reflexivity.
-             ++ rewrite free_variables_noop_substitute; cycle 1.
+          destruct (x ∈ FV t) eqn:?.
+          -- rewrite FV_after_substitute // in_fsetU in_fsetD in_fset1 H1 andbT n /=.
+             destruct (y ∈ FV t) eqn:?.
+             ++ rewrite FV_after_substitute // in_fsetU in_fsetD in_fset1 H1 n0. reflexivity.
+             ++ rewrite FV_noop_substitute; cycle 1.
                 { rewrite Heqb0 //. }
                 rewrite H1. reflexivity.
-          -- rewrite free_variables_noop_substitute; cycle 1.
+          -- rewrite FV_noop_substitute; cycle 1.
              { rewrite Heqb //. }
              rewrite H1.
-             destruct (y \in FV t) eqn:?.
-             ++ rewrite free_variables_after_substitute // in_fsetU in_fsetD in_fset1 H1 andbT n0. reflexivity.
-             ++ rewrite free_variables_noop_substitute; cycle 1.
+             destruct (y ∈ FV t) eqn:?.
+             ++ rewrite FV_after_substitute // in_fsetU in_fsetD in_fset1 H1 andbT n0. reflexivity.
+             ++ rewrite FV_noop_substitute; cycle 1.
                 { rewrite Heqb0 //. }
                 rewrite H1. reflexivity.
   Qed.
@@ -2091,9 +2113,10 @@ Module AlphaFacts (Import M : Alpha).
 
   Implicit Types (c d i j n : nat) (ϕ ψ : {fmap 𝒱 → nat}).
 
+  Definition nat_to_pred n i : bool := i < n.
+
   (** Page 7: "Here we identify n ∈ Nat with the set {i ∈ Nat | i < n}." *)
-  #[global] Instance nat_HasMembers : HasMembers nat nat bool :=
-    { is_member_of i n := i < n }.
+  Canonical nat_predType := PredType nat_to_pred.
 
   Inductive de_Bruijn_term : Type :=
   | de_Bruijn_abstraction : de_Bruijn_term -> de_Bruijn_term
@@ -2122,7 +2145,7 @@ Module AlphaFacts (Import M : Alpha).
 
     Inductive in_de_Bruijn_Tm : nat -> de_Bruijn_term -> Prop :=
     | de_Bruijn_Tm_variable : forall n i,
-        i ∈ n : Prop ->
+        i ∈ n ->
         i ∈ Tm^db n
     | de_Bruijn_Tm_application : forall n dBt dBu,
         dBt ∈ Tm^db n ->
@@ -2137,8 +2160,9 @@ Module AlphaFacts (Import M : Alpha).
 
   Lemma de_Bruijn_TmP : forall n dBt, reflect (in_de_Bruijn_Tm n dBt) (dBt ∈ Tm^db n).
   Proof.
+    rewrite /in_mem /=.
     simpl. intros.
-    gen n. induction dBt; simpl; intros.
+    gen n. induction dBt; simpl; intros; rewrite /in_mem /=.
     - destruct (IHdBt n.+1); repeat constructor.
       + rewrite addn1 //.
       + intros_all. apply n0. inverts H. rewrite addn1 // in H2.
@@ -2146,28 +2170,32 @@ Module AlphaFacts (Import M : Alpha).
       + destruct (IHdBt2 n); repeat constructor; auto.
         intros_all. apply n0. inverts H. auto.
       + intros_all. inverts H. auto.
-    - gen n0. induction n; intros;
+    - rewrite /nat_to_pred.
+      gen n0. induction n; intros;
       destruct n0; repeat constructor; intros_all; simpl in *;
       try solve [inverts H; inverts H2].
       replace (n.+1 < n0.+1) with (n < n0) by auto.
       (pose proof (IHn n0)); inverts H; repeat constructor.
       { simpl. auto. }
       intros_all. inverts H. simpl in *.
+      rewrite /in_mem /= /nat_to_pred in H4.
       replace (n.+1 < n0.+1) with (n < n0) in H4 by auto.
       rewrite H4 // in H0.
   Qed.
 
   Lemma de_Bruijn_Tm_subset :
-    forall n n',
+    forall n n' dBt,
       n <= n' ->
-      Tm^db n ⊆ Tm^db n'.
+      dBt ∈ Tm^db n ->
+      dBt ∈ Tm^db n'.
   Proof.
-    simpl. intros.
-    gen n n'. induction a; intros; simpl in *.
-    - apply IHa with (n.+1); auto.
+    rewrite /in_mem /=.
+    intros.
+    gen n n'. induction dBt; intros; simpl in *.
+    - apply IHdBt with (n.+1); auto.
     - apply (rwP andP) in H0 as [].
-      eapply IHa1 with (n' := n') in H0; auto. eapply IHa2 with (n' := n') in H1; auto.
-      rewrite H0 H1 //.
+      eapply IHdBt1 with (n' := n') in H0; auto. eapply IHdBt2 with (n' := n') in H1; auto.
+      rewrite /in_mem /= H0 H1 //.
     - apply leq_trans with n0; auto.
   Qed.
 
@@ -2179,40 +2207,10 @@ Module AlphaFacts (Import M : Alpha).
   Definition codomm_𝐍 ϕ : nat :=
     S (\max_(i <- codomm ϕ) i).
 
-  (* TODO Move to [FiniteStructures]. *)
-  Lemma remm_mapm :
-    forall (f : nat -> nat) ϕ x,
-      remm (mapm f ϕ) x = mapm f (remm ϕ x).
-  Proof.
-    intros.
-    apply eq_fmap. intros_all.
-    rewrite remmE !mapmE remmE.
-    destruct (x0 =P x); subst; auto.
-  Qed.
-
-  (* TODO Move to [FiniteStructures]. *)
-  Lemma codomm_mapm :
-    forall (f : nat -> nat) ϕ,
-      codomm (mapm f ϕ) = f @: codomm ϕ.
-  Proof.
-    intros.
-    apply eq_fset. intros_all.
-    apply Bool.eq_iff_eq_true. split; intros.
-    - apply (rwP codommP) in H as [].
-      rewrite mapmE in H.
-      destruct (getm ϕ x0) eqn:?; inverts H.
-      apply (rwP imfsetP). exists n; auto.
-      apply (rwP codommP). eauto.
-    - apply (rwP imfsetP) in H as [].
-      apply (rwP codommP) in H as [].
-      subst.
-      apply (rwP codommP).
-      exists x1. rewrite mapmE H //.
-  Qed.
-
   Lemma ϕ_type :
-    forall ϕ,
-      codomm ϕ ⊆ codomm_𝐍 ϕ.
+    forall ϕ n,
+      n ∈ codomm ϕ ->
+      n ∈ codomm_𝐍 ϕ.
   Proof.
     intros. rewrite /codomm_𝐍 -maxE. apply maximum_correct. auto.
   Qed.
@@ -2225,38 +2223,9 @@ Module AlphaFacts (Import M : Alpha).
     rewrite domm_set domm_map fsetUC //.
   Qed.
 
-  (* TODO Move to [Util]. *)
-  Lemma bigmax_subset :
-    forall sub super : seq nat,
-      sub ⊆ super ->
-      \max_(x <- sub) x <= \max_(x <- super) x.
-  Proof.
-    intros.
-    gen super. induction sub; intros; simpl in *.
-    - rewrite big_nil //.
-    - rewrite big_cons.
-      assert (a \in a :: sub). { rewrite in_cons eq_refl //. }
-      apply H in H0.
-      rewrite geq_max -{1}maxE maximum_correct //.
-      apply IHsub. intros.
-      apply H. rewrite in_cons.
-      destruct (a0 =P a); subst; auto.
-  Qed.
-
-  (* TODO Move to [Util]. *)
-  Lemma S_bigmax :
-    forall s : seq nat,
-      \max_(x <- s) S x <= S (\max_(x <- s) x).
-  Proof.
-    intros.
-    induction s.
-    { rewrite !big_nil //. }
-    rewrite !big_cons -!maxnSS geq_max leq_max leqnn leq_max IHs orbT //.
-  Qed.
-
   Lemma codomm_𝐍_update_ϕ :
     forall ϕ x,
-      codomm_𝐍 (ϕ^+x) <= S (codomm_𝐍 ϕ) : Prop.
+      codomm_𝐍 (ϕ^+x) <= S (codomm_𝐍 ϕ).
   Proof.
     unfold codomm_𝐍.
     intros.
@@ -2270,21 +2239,21 @@ Module AlphaFacts (Import M : Alpha).
 
   Lemma codomm_update_ϕ :
     forall ϕ x,
-      codomm (ϕ^+x) ⊆ S (codomm_𝐍 ϕ) : Prop.
+      {subset codomm (ϕ^+x) <= S (codomm_𝐍 ϕ)}.
   Proof.
-    simpl. intros.
+    intros_all.
     apply (rwP codommP) in H as [].
     rewrite setmE mapmE in H.
-    destruct (x0 =P x); subst.
+    destruct (x1 =P x); subst.
     { inverts H. auto. }
-    destruct (getm ϕ x0) eqn:?; inverts H.
+    destruct (getm ϕ x1) eqn:?; inverts H.
     apply ϕ_type. simpl. apply (rwP codommP). eauto.
   Qed.
 
   (** Page 8: "where ϕ^+x(y) = ...." *)
   Lemma update_ϕ_correct :
     forall ϕ x y,
-      y ∈ domm ϕ ∪ {x} : Prop ->
+      y ∈ domm ϕ ∪ {x} ->
       getm (ϕ^+x) y =
       if y == x
       then Some 0
@@ -2339,22 +2308,24 @@ Module AlphaFacts (Import M : Alpha).
   (** Page 8: "t^ϕ ∈ Tm^db(n)". *)
   Lemma to_de_Bruijn_type :
     forall ϕ t,
-      FV t ⊆ domm ϕ ->
-      t^ϕ ∈ Tm^db (codomm_𝐍 ϕ) : Prop.
+      t ∈ Tm (domm ϕ) ->
+      t^ϕ ∈ Tm^db (codomm_𝐍 ϕ).
   Proof.
+    rewrite /in_mem /= /Tm.
     intros.
+    apply (rwP fsubsetP) in H.
     gen ϕ. induction t; intros; simpl in *.
     - apply de_Bruijn_Tm_subset with (codomm_𝐍 (ϕ^+s)).
       + apply codomm_𝐍_update_ϕ.
-      + apply IHt. simpl. intros.
+      + apply IHt. intros_all.
         rewrite domm_set domm_map in_fsetU in_fset1.
-        destruct (a =P s); subst; auto.
+        destruct (x =P s); subst; auto.
         apply (introF eqP) in n.
         apply H. rewrite in_fsetD in_fset1 n H0 //.
     - apply (rwP (@andP (Tm^db _ _) (Tm^db _ _))). split;
-      (apply IHt1 || apply IHt2); simpl; intros;
+      (apply IHt1 || apply IHt2); simpl; intros_all;
       apply H; rewrite in_fsetU H0 ?orbT //.
-    - assert (s \in fset1 s). { rewrite in_fset1 eq_refl //. }
+    - assert (s ∈ fset1 s). { rewrite in_fset1 eq_refl //. }
       apply H, (rwP dommP) in H0 as []. rewrite H0.
       apply ϕ_type, (rwP codommP). eauto.
   Qed.
@@ -2380,7 +2351,7 @@ Module AlphaFacts (Import M : Alpha).
       destruct (getm R x0) eqn:?; cycle 1.
       { inverts H3. }
       destruct (y =P s); subst; inverts H3.
-      pose proof Heqo. apply H in Heqo as [].
+      pose proof Heqo. apply H, (rwP andP) in Heqo as [].
       simpl in *. apply (rwP dommP) in H4 as [].
       apply (rwP dommP) in H5 as [].
       apply not_eq_sym, (introF eqP) in n0.
@@ -2395,7 +2366,7 @@ Module AlphaFacts (Import M : Alpha).
         destruct (getm ψ y0) eqn:?; inverts H4.
       + destruct (getm R x0) eqn:?.
         * pose proof Heqo.
-          apply H in H5 as [].
+          apply H, (rwP andP) in H5 as [].
           simpl in *. apply (rwP dommP) in H5 as [].
           apply (rwP dommP) in H6 as [].
           rewrite H5 in H4.
@@ -2410,8 +2381,8 @@ Module AlphaFacts (Import M : Alpha).
           destruct (y0 =P y); subst; inverts H4.
           -- destruct (getm ψ y0) eqn:?; inverts H6.
              rewrite -Heqo1 in Heqo0.
-             assert (x0 \in domm ϕ). { apply (rwP dommP). rewrite Heqo0 Heqo1. eauto. }
-             assert (x0 \in domm ϕ /\ getm ϕ x0 = getm ψ y0) by auto.
+             assert (x0 ∈ domm ϕ). { apply (rwP dommP). rewrite Heqo0 Heqo1. eauto. }
+             assert (x0 ∈ domm ϕ /\ getm ϕ x0 = getm ψ y0) by auto.
              apply H2 in H5. rewrite H5 // in Heqo.
           -- destruct (getm ψ y0) eqn:?; inverts H6.
              rewrite -Heqo1 in Heqo0.
@@ -2427,63 +2398,66 @@ Module AlphaFacts (Import M : Alpha).
       is_injective ϕ ->
       is_injective ψ ->
       is_pullback R ϕ ψ ->
-      FV t ⊆ domm ϕ ->
-      FV u ⊆ domm ψ ->
+      t ∈ Tm (domm ϕ) ->
+      u ∈ Tm (domm ψ) ->
       t ≡_α^R u <-> t^ϕ = u^ψ.
   Proof.
     intros.
+    apply (rwP fsubsetP) in H3, H4.
     gen R ϕ ψ u. induction t; intros; split; intros;
     destruct u; inverts H5; simpl in *.
     - f_equal.
-      eapply IHt; eauto; intros.
+      eapply IHt; eauto; intros_all.
       + apply injective_update_ϕ. auto.
       + rewrite domm_update_ϕ in_fsetU in_fset1 orbC.
-        destruct (a =P s); subst; auto.
+        destruct (x =P s); subst; auto.
         apply (introF eqP) in n.
         apply H3. rewrite in_fsetD in_fset1 n H5 //.
-      + rewrite !domm_update_ϕ. apply update_type; auto.
+      + rewrite !domm_update_ϕ. eapply update_type; eauto.
+        intros. apply (rwP andP). auto.
       + apply injective_update_ϕ. auto.
       + apply lemma9'; simpl; eauto.
       + rewrite domm_update_ϕ in_fsetU in_fset1 orbC.
-        destruct (a =P s0); subst; auto.
+        destruct (x =P s0); subst; auto.
         apply (introF eqP) in n.
         apply H4. rewrite in_fsetD in_fset1 n H5 //.
-    - eapply IHt in H7; eauto; intros.
+    - eapply IHt in H7; eauto; intros_all.
       + apply injective_update_ϕ. auto.
       + rewrite domm_update_ϕ in_fsetU in_fset1 orbC.
-        destruct (a =P s); subst; auto.
+        destruct (x =P s); subst; auto.
         apply (introF eqP) in n.
         apply H3. rewrite in_fsetD in_fset1 n H6 //.
-      + rewrite !domm_update_ϕ. apply update_type; auto.
+      + rewrite !domm_update_ϕ. eapply update_type; eauto.
+        intros. apply (rwP andP). auto.
       + apply injective_update_ϕ. auto.
       + apply lemma9'; simpl; eauto.
       + rewrite domm_update_ϕ in_fsetU in_fset1 orbC.
-        destruct (a =P s0); subst; auto.
+        destruct (x =P s0); subst; auto.
         apply (introF eqP) in n.
         apply H4. rewrite in_fsetD in_fset1 n H6 //.
     - apply (rwP andP) in H7 as [].
-      eapply IHt1 with (ϕ := ϕ) (ψ := ψ) in H5; cycle 1; intros; eauto.
+      eapply IHt1 with (ϕ := ϕ) (ψ := ψ) in H5; cycle 1; intros_all; eauto.
       { apply H3. rewrite in_fsetU H8 //. }
       { apply H4. rewrite in_fsetU H8 //. }
-      eapply IHt2 with (ϕ := ϕ) (ψ := ψ) in H6; cycle 1; intros; eauto.
+      eapply IHt2 with (ϕ := ϕ) (ψ := ψ) in H6; cycle 1; intros_all; eauto.
       { apply H3. rewrite in_fsetU H8 orbT //. }
       { apply H4. rewrite in_fsetU H8 orbT //. }
       rewrite H5 H6 //.
-    - eapply IHt1 in H7; cycle 1; intros; eauto.
+    - eapply IHt1 in H7; cycle 1; intros_all; eauto.
       { apply H3. rewrite in_fsetU H6 //. }
       { apply H4. rewrite in_fsetU H6 //. }
-      eapply IHt2 in H8; cycle 1; intros; eauto.
+      eapply IHt2 in H8; cycle 1; intros_all; eauto.
       { apply H3. rewrite in_fsetU H6 orbT //. }
       { apply H4. rewrite in_fsetU H6 orbT //. }
       rewrite H7 H8 //.
-    - apply (rwP eqP) in H7.
+    - apply (rwP (getmP _ _ _)) in H7.
       apply H2 in H7 as [].
       simpl in *. apply (rwP dommP) in H5 as [].
       rewrite H5 in H6. rewrite H5 -H6 //.
-    - rewrite <- (rwP eqP).
-      assert (s \in fset1 s). { rewrite in_fset1 //. }
+    - rewrite <- (rwP (getmP _ _ _)).
+      assert (s ∈ fset1 s). { rewrite in_fset1 //. }
       apply H3, (rwP dommP) in H5 as [].
-      assert (s0 \in fset1 s0). { rewrite in_fset1 //. }
+      assert (s0 ∈ fset1 s0). { rewrite in_fset1 //. }
       apply H4, (rwP dommP) in H6 as [].
       rewrite H5 H6 /= in H7. subst.
       apply H2. split.
@@ -2499,9 +2473,9 @@ Module AlphaFacts (Import M : Alpha).
     intros.
     repeat (split; intros).
     - rewrite /fmap_to_Prop mkfmapfE in H0.
-      destruct (x \in domm ϕ) eqn:?; rewrite Heqb in H0; inverts H0. auto.
+      destruct (x ∈ domm ϕ) eqn:?; rewrite Heqb in H0; inverts H0. auto.
     - rewrite /fmap_to_Prop mkfmapfE in H0.
-      destruct (x \in domm ϕ) eqn:?; rewrite Heqb in H0; inverts H0. auto.
+      destruct (x ∈ domm ϕ) eqn:?; rewrite Heqb in H0; inverts H0. auto.
     - destruct H0.
       simpl in *. rewrite /fmap_to_Prop mkfmapfE H0.
       apply (rwP (injectivemP _)) in H0; auto.
@@ -2512,19 +2486,19 @@ Module AlphaFacts (Import M : Alpha).
   Proposition to_de_Bruijn_chooses_canonical_representations :
     forall t u ϕ,
       is_injective ϕ ->
-      t ∈ Tm (domm ϕ) : Prop ->
-      u ∈ Tm (domm ϕ) : Prop ->
+      t ∈ Tm (domm ϕ) ->
+      u ∈ Tm (domm ϕ) ->
       t ≡_α u <-> t^ϕ = u^ϕ.
   Proof.
     intros.
-    unfold Tm in *. apply (rwP fsubsetP) in H0, H1.
     split; intros.
     - apply lemma9 with (R := 1__(domm ϕ)); auto.
       + apply identity_type.
       + apply identity_is_pullback. auto.
       + apply α_equivalent'_supermap with (R__sub := 1__(FV t)); auto. intros.
         rewrite mkfmapfE in H3.
-        destruct (k \in FV t) eqn:?; rewrite Heqb in H3; inverts H3.
+        destruct (k ∈ FV t) eqn:?; rewrite Heqb in H3; inverts H3.
+        apply (rwP fsubsetP) in H0.
         apply H0 in Heqb.
         rewrite mkfmapfE Heqb //.
     - eapply lemma9 with (R := 1__(domm ϕ)) in H2; auto.
@@ -2559,16 +2533,18 @@ Module AlphaFacts (Import M : Alpha).
 
   Lemma TAPL_6_2_3 :
     forall n dBt c d,
-      dBt ∈ Tm^db n : Prop ->
-      ↑_c^d dBt ∈ Tm^db (n + d) : Prop.
+      dBt ∈ Tm^db n ->
+      ↑_c^d dBt ∈ Tm^db (n + d).
   Proof.
+    rewrite /in_mem /=.
     intros.
-    gen n c d. induction dBt; intros; simpl in *.
+    gen n c d. induction dBt; intros; repeat rewrite /in_mem /=.
     - eapply IHdBt in H; eauto.
     - apply (rwP andP) in H as [].
       rewrite <- (rwP (@andP (Tm^db (n + d) (↑_c^d dBt1)) (Tm^db (n + d) (↑_c^d dBt2)))).
       split; eauto.
-    - destruct (n < c) eqn:?.
+    - rewrite /nat_to_pred.
+      destruct (n < c) eqn:?.
       + rewrite ltn_addr //.
       + rewrite ltn_add2r //.
   Qed.
@@ -2701,10 +2677,10 @@ Module AlphaFacts (Import M : Alpha).
 
   Lemma TAPL_6_2_6 :
     forall j n dBt dBu,
-      dBt ∈ Tm^db n : Prop ->
-      dBu ∈ Tm^db n : Prop ->
+      dBt ∈ Tm^db n ->
+      dBu ∈ Tm^db n ->
       j <= n ->
-      [j↦dBu]dBt ∈ Tm^db n : Prop.
+      [j↦dBu]dBt ∈ Tm^db n.
   Proof.
     intros.
     gen j n dBu. induction dBt; intros; simpl in *.
@@ -2715,7 +2691,7 @@ Module AlphaFacts (Import M : Alpha).
     - apply (rwP andP) in H as [].
       eapply IHdBt1 with (dBu := dBu) in H; eauto.
       eapply IHdBt2 with (dBu := dBu) in H2; eauto.
-      rewrite H H2 //.
+      rewrite /in_mem /= H H2 //.
     - destruct (n =P j); subst; auto.
   Qed.
 
@@ -2729,7 +2705,7 @@ Module AlphaFacts (Import M : Alpha).
     - apply (rwP codomm_Tm_setP) in H as (? & ? & ?).
       simpl in *. apply (rwP codommP) in H0 as [].
       rewrite mapmE mkfmapfE in H0.
-      destruct (x1 \in X) eqn:?; rewrite Heqb in H0; inverts H0.
+      destruct (x1 ∈ X) eqn:?; rewrite Heqb in H0; inverts H0.
       rewrite in_fset1 in H. apply (rwP eqP) in H. subst. auto.
     - apply (rwP codomm_Tm_setP).
       exists (variable x). split.
@@ -2753,7 +2729,7 @@ Module AlphaFacts (Import M : Alpha).
     { apply eq_fmap. intros_all.
       rewrite setmE !mapmE mkfmapfE unionmE remmE rem_valmE setmE /= mkfmapfE.
       destruct (x0 =P x); subst; auto.
-      destruct (x0 \in FV t) eqn:?; rewrite Heqb //.
+      destruct (x0 ∈ FV t) eqn:?; rewrite Heqb //.
       destruct (y =P x0); subst; auto.
       rewrite Heqb // in H. }
     replace ((identity (FV t :\ x))⦅x,y⦆ᵒ) with ((identity (FV t))⦅x,y⦆ᵒ); cycle 1.
@@ -2763,25 +2739,25 @@ Module AlphaFacts (Import M : Alpha).
         destruct (x0 =P y); subst; auto.
         rewrite !converse_identity !mkfmapfE !in_fsetD !in_fset1.
         destruct (x0 =P x); subst; auto.
-        destruct (x \in FV t) eqn:?; rewrite Heqb // eq_refl //.
+        destruct (x ∈ FV t) eqn:?; rewrite Heqb // eq_refl //.
       - apply partial_bijection_identity.
       - apply partial_bijection_identity. }
     apply lemma7.
     - apply partial_bijection_update, partial_bijection_identity.
-    - simpl. intros.
+    - rewrite /Tm /in_mem /=. apply (rwP fsubsetP). intros_all.
       apply (rwP dommP).
       rewrite unionmE remmE rem_valmE setmE /= mkfmapfE.
-      destruct (a =P x); subst; simpl; eauto.
+      destruct (x0 =P x); subst; simpl; eauto.
       rewrite H0.
-      destruct (y =P a); subst; simpl; eauto.
+      destruct (y =P x0); subst; simpl; eauto.
       rewrite H0 // in H.
   Qed.
 
   Lemma update_as_update_ϕ :
     forall t u x y ϕ,
       is_injective ϕ ->
-      t ∈ Tm (domm ϕ ∪ {y}) : Prop ->
-      u ∈ Tm (domm ϕ ∪ {x}) : Prop ->
+      t ∈ Tm (domm ϕ ∪ {y}) ->
+      u ∈ Tm (domm ϕ ∪ {x}) ->
       t ≡_α^(1__(domm ϕ))⦅y,x⦆ u ->
       t^ϕ^+y = u^ϕ^+x.
   Proof.
@@ -2792,7 +2768,7 @@ Module AlphaFacts (Import M : Alpha).
     - rewrite !domm_set ![_ |: _]fsetUC. apply update_type.
       + simpl. intros.
         rewrite /fmap_to_Prop mkfmapfE in H3.
-        destruct (a \in domm ϕ) eqn:?; rewrite Heqb0 in H3; inverts H3.
+        destruct (a ∈ domm ϕ) eqn:?; rewrite Heqb0 in H3; inverts H3.
         rewrite domm_map Heqb0 //.
       + rewrite domm_map. apply identity_type.
     - apply injective_update_ϕ. auto.
@@ -2800,13 +2776,13 @@ Module AlphaFacts (Import M : Alpha).
     - eapply lemma9'; eauto.
       + apply identity_type.
       + eapply identity_is_pullback; eauto.
-    - rewrite domm_set domm_map /= fsetUC. intros. apply H0. auto.
-    - rewrite domm_set domm_map /= fsetUC. intros. apply H1. auto.
+    - rewrite /Tm /in_mem domm_set domm_map /= fsetUC. apply (rwP fsubsetP). intros_all. apply H0. auto.
+    - rewrite /Tm /in_mem domm_set domm_map /= fsetUC. apply (rwP fsubsetP). intros_all. apply H1. auto.
   Qed.
 
   Lemma to_de_Bruijn_with_indistinguishable_ϕ :
     forall ϕ ψ t,
-      (forall x, x ∈ FV t : Prop -> getm ϕ x = getm ψ x) ->
+      (forall x, x ∈ FV t -> getm ϕ x = getm ψ x) ->
       t^ϕ = t^ψ.
   Proof.
     intros.
@@ -2842,12 +2818,13 @@ Module AlphaFacts (Import M : Alpha).
       t[x⟵variable x] ≡_α t.
   Proof.
     intros.
-    destruct (x \in FV t) eqn:?; cycle 1.
+    destruct (x ∈ FV t) eqn:?; cycle 1.
     { apply substitution_law1. rewrite Heqb //. }
     transitivity (⦇η__(FV t)⦈ t); cycle 1.
-    { apply monad_substitution1. auto. }
+    { apply monad_substitution1. rewrite /Tm /in_mem /=. apply (rwP fsubsetP). intros_all. auto. }
     apply lift_substitution_indistinguishable_substitutions; simpl; intros.
-    - rewrite in_fsetI !domm_set domm_map !domm_mkfmapf !in_fsetU !in_fset1 !in_fset orbC H //.
+    - rewrite /in_mem /Tm /=. apply (rwP fsubsetP). intros_all.
+      rewrite in_fsetI !domm_set domm_map !domm_mkfmapf !in_fsetU !in_fset1 !in_fset orbC H //.
     - rewrite setmE mapmE mkfmapfE H.
       destruct (x0 =P x); subst; reflexivity.
   Qed.
@@ -2871,7 +2848,7 @@ Module AlphaFacts (Import M : Alpha).
   Lemma substitution_as_update_ϕ :
     forall ϕ t x y,
       is_injective ϕ ->
-      t ∈ Tm (domm ϕ) : Prop ->
+      t ∈ Tm (domm ϕ) ->
       y ∉ FV t ->
       (t[x⟵variable y])^ϕ^+y = t^ϕ^+x.
   Proof.
@@ -2881,26 +2858,26 @@ Module AlphaFacts (Import M : Alpha).
     destruct (x =P y); subst.
     { apply to_de_Bruijn_chooses_canonical_representations.
       - apply injective_update_ϕ. auto.
-      - rewrite /Tm /=. apply (rwP fsubsetP). intros_all.
-        rewrite free_variables_noop_substitute // in H2.
+      - rewrite /Tm /in_mem /=. apply (rwP fsubsetP). intros_all.
+        rewrite FV_noop_substitute // in H2.
         apply H0 in H2.
         rewrite domm_set domm_map in_fsetU in_fset1 orbC H2 //.
-      - rewrite /Tm /=. apply (rwP fsubsetP). intros_all.
+      - rewrite /Tm /in_mem /=. apply (rwP fsubsetP). intros_all.
         apply H0 in H2.
         rewrite domm_set domm_map in_fsetU in_fset1 orbC H2 //.
       - apply substitution_id. }
     eapply update_as_update_ϕ; eauto.
-    - rewrite /Tm /=. apply (rwP fsubsetP). intros_all.
+    - rewrite /Tm /in_mem /=. apply (rwP fsubsetP). intros_all.
       rewrite in_fsetU in_fset1 orbC.
       destruct (x0 =P y); subst; auto.
       apply H0.
-      destruct (x \in FV t) eqn:?.
-      + rewrite free_variables_after_substitute // in_fsetU in_fsetD !in_fset1 in H2.
+      destruct (x ∈ FV t) eqn:?.
+      + rewrite FV_after_substitute // in_fsetU in_fsetD !in_fset1 in H2.
         apply (rwP orP) in H2 as [].
         * apply (rwP andP) in H2 as []. auto.
         * apply (rwP eqP) in H2. subst. contradiction.
-      + rewrite free_variables_noop_substitute // Heqb // in H2.
-    - rewrite /Tm /=. apply (rwP fsubsetP). intros_all.
+      + rewrite FV_noop_substitute // Heqb // in H2.
+    - rewrite /Tm /in_mem /=. apply (rwP fsubsetP). intros_all.
       apply H0 in H2.
       rewrite in_fsetU in_fset1 H2 //.
     - apply α_equivalent'_supermap with (R__sub := (1__(FV t :\ x))⦅y,x⦆).
@@ -2910,7 +2887,7 @@ Module AlphaFacts (Import M : Alpha).
         destruct (k =P y); subst; auto.
         destruct (k =P x); subst.
         { inverts H2. }
-        destruct (k \in FV t) eqn:?; cycle 1.
+        destruct (k ∈ FV t) eqn:?; cycle 1.
         { inverts H2. }
         simpl in *.
         destruct (x =P k); subst; inverts H2.
@@ -2959,19 +2936,20 @@ Module AlphaFacts (Import M : Alpha).
 
   Lemma noop_de_Bruijn_substitution :
     forall ϕ i t dBu,
-      FV t ⊆ domm ϕ ->
+      t ∈ Tm (domm ϕ) ->
       i ∉ codomm ϕ ->
       let dBt := t^ϕ in
       [i↦dBu]dBt = dBt.
   Proof.
     intros.
     subst dBt.
+    apply (rwP fsubsetP) in H.
     rewrite <- (rwP (@codommPn _ _ ϕ i)) in H0.
     gen ϕ i dBu. induction t; intros;
     simpl; f_equal.
-    - apply IHt; simpl; intros.
+    - apply IHt; simpl; intros_all.
       { rewrite domm_set domm_mapi in_fsetU in_fset1.
-        destruct (a =P s); subst; auto.
+        destruct (x =P s); subst; auto.
         simpl in *. apply H.
         apply (introF eqP) in n.
         rewrite in_fsetD in_fset1 n H1 //. }
@@ -2979,9 +2957,9 @@ Module AlphaFacts (Import M : Alpha).
       destruct (k' =P s); subst; auto.
       destruct (getm ϕ k') eqn:?; auto.
       pose proof H0 k'. rewrite Heqo // in H1.
-    - apply IHt1; auto. simpl in *. intros.
+    - apply IHt1; auto. simpl in *. intros_all.
       apply H. rewrite in_fsetU H1 //.
-    - apply IHt2; auto. simpl in *. intros.
+    - apply IHt2; auto. simpl in *. intros_all.
       apply H. rewrite in_fsetU H1 orbT //.
     - destruct (getm ϕ s) eqn:?.
       + pose proof H0 s. rewrite Heqo in H1.
@@ -2998,33 +2976,35 @@ Module AlphaFacts (Import M : Alpha).
     predn @: (s :\ 0).
 
   (* TODO Overload [FV] notation to include this. *)
-  Fixpoint de_Bruijn_free_variables dBt : {fset nat} :=
+  Fixpoint de_Bruijn_FV dBt : {fset nat} :=
     match dBt with
     | de_Bruijn_abstraction dBt =>
-      decr (de_Bruijn_free_variables dBt)
+      decr (de_Bruijn_FV dBt)
     | de_Bruijn_application dBt1 dBt2 =>
-      de_Bruijn_free_variables dBt1 ∪ de_Bruijn_free_variables dBt2
+      de_Bruijn_FV dBt1 ∪ de_Bruijn_FV dBt2
     | de_Bruijn_variable n =>
       fset1 n
     end.
 
-  #[local] Notation FV' := de_Bruijn_free_variables.
+  #[local] Notation FV' := de_Bruijn_FV.
 
   Lemma FV'_as_FV :
     forall ϕ t,
-      FV t ⊆ domm ϕ ->
+      t ∈ Tm (domm ϕ) ->
       FV' (t^ϕ) = pimfset (getm ϕ) (FV t).
   Proof.
     intros.
+    apply (rwP fsubsetP) in H.
     apply eq_fset. intros_all.
     gen x ϕ. induction t; intros; simpl in *.
-    - assert (FV t ⊆ domm (ϕ^+s)).
-      { simpl. intros.
+    - assert (t ∈ Tm (domm (ϕ^+s))).
+      { rewrite /Tm /in_mem /=. apply (rwP fsubsetP). intros_all.
         rewrite domm_set domm_mapi in_fsetU in_fset1.
-        destruct (a =P s); subst; auto.
+        destruct (x0 =P s); subst; auto.
         apply H.
         apply (introF eqP) in n.
         rewrite in_fsetD in_fset1 n H0 //. }
+      apply (rwP fsubsetP) in H0.
       pose proof (fun i => @IHt i _ H0).
       apply Bool.eq_iff_eq_true. split; intros.
       + apply (rwP (pimfsetP _ _ _)).
@@ -3040,7 +3020,7 @@ Module AlphaFacts (Import M : Alpha).
         destruct (x =P s); subst.
         { inverts H3. }
         apply (introF eqP) in n.
-        assert (x \in domm ϕ).
+        assert (x ∈ domm ϕ).
         { apply H. rewrite in_fsetD in_fset1 n H2 //. }
         apply (rwP dommP) in H5 as [].
         rewrite H5 in H3. inverts H3.
@@ -3061,24 +3041,24 @@ Module AlphaFacts (Import M : Alpha).
         * rewrite IHt1 in H0.
           -- apply (rwP (pimfsetP _ _ _)) in H0 as [].
              exists x0; auto. rewrite in_fsetU H0 //.
-          -- intros. apply H. rewrite in_fsetU H0 //.
+          -- intros_all. apply H. rewrite in_fsetU H0 //.
         * rewrite IHt2 in H0.
           -- apply (rwP (pimfsetP _ _ _)) in H0 as [].
              exists x0; auto. rewrite in_fsetU H0 orbT //.
-          -- intros. apply H. rewrite in_fsetU H0 orbT //.
+          -- intros_all. apply H. rewrite in_fsetU H0 orbT //.
       + apply (rwP orP).
         apply (rwP (pimfsetP _ _ _)) in H0 as [].
         rewrite in_fsetU in H0. apply (rwP orP) in H0 as [].
         * left. rewrite IHt1.
           -- apply (rwP (pimfsetP _ _ _)). eauto.
-          -- intros. apply H. rewrite in_fsetU H2 //.
+          -- intros_all. apply H. rewrite in_fsetU H2 //.
         * right. rewrite IHt2.
           -- apply (rwP (pimfsetP _ _ _)). eauto.
-          -- intros. apply H. rewrite in_fsetU H2 orbT //.
+          -- intros_all. apply H. rewrite in_fsetU H2 orbT //.
     - rewrite in_fset1.
       apply Bool.eq_iff_eq_true. split; intros.
       + apply (rwP eqP) in H0. subst.
-        assert (s \in domm ϕ). { apply H. rewrite in_fset1 eq_refl //. }
+        assert (s ∈ domm ϕ). { apply H. rewrite in_fset1 eq_refl //. }
         apply (rwP dommP) in H0 as [].
         apply (rwP (pimfsetP _ (fset1 s) _)). exists s.
         * rewrite in_fset1 eq_refl //.
@@ -3091,7 +3071,7 @@ Module AlphaFacts (Import M : Alpha).
   Lemma noop_de_Bruijn_substitution' :
     forall ϕ i x t dBu,
       is_injective ϕ ->
-      FV t ⊆ domm ϕ ->
+      t ∈ Tm (domm ϕ) ->
       getm ϕ x = Some i ->
       x ∉ FV t ->
       let dBt := t^ϕ in
@@ -3099,6 +3079,7 @@ Module AlphaFacts (Import M : Alpha).
   Proof.
     intros.
     subst dBt.
+    apply (rwP fsubsetP) in H0.
     gen ϕ x i dBu. induction t; intros;
     simpl in *.
     - f_equal.
@@ -3106,9 +3087,9 @@ Module AlphaFacts (Import M : Alpha).
       destruct (x =P s); subst.
       + pose proof old_index_after_update_ϕ _ H H1.
         apply noop_de_Bruijn_substitution.
-        * simpl. intros.
+        * rewrite /Tm /in_mem /=. apply (rwP fsubsetP). intros_all.
           rewrite domm_set domm_mapi in_fsetU in_fset1.
-          destruct (a =P s); subst; auto.
+          destruct (x =P s); subst; auto.
           apply (introF eqP) in n.
           apply H0. rewrite in_fsetD in_fset1 n H4 //.
         * rewrite <- (rwP (@codommPn _ _ (ϕ^+s) _)). intros.
@@ -3118,19 +3099,19 @@ Module AlphaFacts (Import M : Alpha).
       + pose proof old_index_after_update_ϕ _ H H1.
         erewrite IHt; eauto.
         * apply injective_update_ϕ. auto.
-        * intros.
+        * intros_all.
           rewrite domm_set domm_mapi in_fsetU in_fset1.
-          destruct (a =P s); subst; auto.
+          destruct (x0 =P s); subst; auto.
           apply (introF eqP) in n0.
           apply H0. rewrite in_fsetD in_fset1 n0 H4 //.
         * apply (introF eqP) in n.
           rewrite setmE mapmE n H1 /= addn1 //.
     - rewrite in_fsetU negb_or in H2. apply (rwP andP) in H2 as [].
       erewrite IHt1; cycle 1; eauto.
-      { intros. apply H0. rewrite in_fsetU H4 //. }
+      { intros_all. apply H0. rewrite in_fsetU H4 //. }
       erewrite IHt2; cycle 1; eauto.
-      intros. apply H0. rewrite in_fsetU H4 orbT //.
-    - assert (s \in domm ϕ). { apply H0. rewrite in_fset1 eq_refl //. }
+      intros_all. apply H0. rewrite in_fsetU H4 orbT //.
+    - assert (s ∈ domm ϕ). { apply H0. rewrite in_fset1 eq_refl //. }
       apply (rwP dommP) in H3 as []. rewrite H3 /=.
       destruct (x0 =P i); subst; auto.
       rewrite -H3 in H1.
@@ -3157,7 +3138,7 @@ Module AlphaFacts (Import M : Alpha).
    *)
   Lemma TAPL_6_2_8 :
     forall ϕ t u x,
-      (FV t ∪ FV u ∪ {x}) ⊆ domm ϕ ->
+      fsubset (FV t ∪ FV u ∪ {x}) (domm ϕ) ->
       is_injective ϕ ->
       (t[x⟵u])^ϕ = [odflt 0 (getm ϕ x)↦u^ϕ](t^ϕ).
   Proof.
