theories/Examples.v
@@ -34,8 +34,20 @@ Example examples :
   (λ"x" λ"x" `"x") ≡_α (λ"y" λ"x" `"x").
 Proof.
   unfold α_equivalent.
-  repeat split; intros_all;
+  repeat split; try apply negbT, Bool.not_true_iff_false; intros_all;
   try apply α_equivalent_iff_α_equivalent'_free_variables;
-  repeat rewrite /= unionmE remmE rem_valmE //=;
-  rewrite mkfmapfE !in_fsetD !in_fsetU //.
+  simpl in *.
+  - apply (rwP (getmP _ _ _)). rewrite unionmE remmE rem_valmE //.
+  - repeat rewrite <- (rwP andP). repeat split;
+    apply (rwP (getmP _ _ _)); repeat rewrite unionmE remmE rem_valmE //=.
+  - repeat rewrite <- (rwP andP). repeat split;
+    apply (rwP (getmP _ _ _)); repeat rewrite unionmE remmE rem_valmE //=.
+    rewrite mkfmapfE !in_fsetD !in_fsetU //.
+  - apply (rwP andP) in H as [].
+    apply (rwP (getmP _ _ _)) in H0.
+    rewrite unionmE remmE rem_valmE /= mkfmapfE !in_fsetD !in_fsetU // in H0.
+  - apply (rwP andP) in H as [].
+    apply (rwP (getmP _ _ _)) in H0.
+    repeat rewrite unionmE remmE rem_valmE // in H0.
+  - apply (rwP (getmP _ _ _)). rewrite unionmE remmE rem_valmE //.
 Qed.
