theories/Util.v
@@ -1,1 +1,1 @@
-From AlphaPearl Require Export Util.Compose Util.FiniteStructures Util.Injective Util.Membership Util.PlfTactics Util.Seq Util.String.
+From AlphaPearl Require Export Util.Compose Util.FiniteStructures Util.Injective Util.PlfTactics Util.Seq Util.String.
