theories/Util/Seq.v
@@ -10,6 +10,10 @@ Unset Printing Implicit Defensive.
 
 #[local] Open Scope list_scope.
 
+Notation "x '∈' y" := (x \in y) (at level 70).
+
+Notation "x '∉' y" := (x \notin y) (at level 70).
+
 (* Note that, at least for now, [maximum nil = 0]. *)
 Definition maximum : list nat -> nat := foldr maxn 0.
 
@@ -23,4 +27,31 @@ Proof.
   - apply IHl in H. rewrite H orbT //.
 Qed.
 
-Lemma maxE r : maximum r = \max_(i <- r) i. Proof. apply foldrE. Qed.
+Lemma maxE r : maximum r = \max_(i <- r) i. Proof. exact: foldrE. Qed.
+
+Lemma bigmax_subset :
+  forall sub super : seq nat,
+    {subset sub <= super} ->
+    \max_(x <- sub) x <= \max_(x <- super) x.
+Proof.
+  intros.
+  gen super. induction sub; intros; simpl in *.
+  - rewrite big_nil //.
+  - rewrite big_cons.
+    assert (a ∈ a :: sub). { rewrite in_cons eq_refl //. }
+    apply H in H0.
+    rewrite geq_max -{1}maxE maximum_correct //.
+    apply IHsub. intros_all.
+    apply H. rewrite in_cons.
+    destruct (x =P a); subst; auto.
+Qed.
+
+Lemma S_bigmax :
+  forall s : seq nat,
+    \max_(x <- s) S x <= S (\max_(x <- s) x).
+Proof.
+  intros.
+  induction s.
+  { rewrite !big_nil //. }
+  rewrite !big_cons -!maxnSS geq_max leq_max leqnn leq_max IHs orbT //.
+Qed.
